proof/correctness1024/MLKEM_PolyVec.ec
@@ -1,13 +1,13 @@
 require import AllCore List IntDiv CoreMap.
 
 from Jasmin require import JModel JMemory.
-from JazzEC require import Array1152 Array960 Array256 Array384 Array128 Array768 Array5.
-from CryptoSpecs require import GFq Rq Serialization VecMat MLKEM768 Correctness768.
+from JazzEC require import Array1152 Array1408 Array1536 Array1568 Array256 Array384 Array128 Array1024 Array5.
+from CryptoSpecs require import GFq Rq Serialization VecMat MLKEM1024 Correctness1024.
 require import W16extra.
 require import Fq MLKEM_Poly NTT_Fq NTTAlgebra MLKEMFCLib.
 
 
-from JazzEC require import Jkem768.
+from JazzEC require import Jkem1024.
 
 theory MLKEM_PolyVec.
 
@@ -16,33 +16,33 @@ import GFq.
 import Zq.
 import MLKEM_Poly.
 import KMatrix.
-import Serialization768.
-import VecMat768.
+import Serialization1024.
+import VecMat1024.
 import PolyVec.
 import PolyMat.
 
 lemma land_foo  p q: p && q <=> p /\ q by smt().
 
-op lift_polyvec(vec: W16.t Array768.t) : polyvec =
+op lift_polyvec(vec: W16.t Array1024.t) : polyvec =
     Vector.offunv (fun i => lift_array256 (subarray256 vec i)).
 
 
 op scale_polyvec(v : polyvec, c : coeff) : polyvec = 
    Vector.offunv (fun i => (scale ((Vector.tofunv v) i) c)).
 
-lemma liftarrayvector a i k : 0<=i<3 => 0<=k<256 =>
-         ((lift_polyvec a).[i])%Vector.[k] = (lift_array768 a).[256*i+k].
-move => ib lb; rewrite /lift_vector /lift_array768 offunvE // mapiE 1:/# /=.
+lemma liftarrayvector a i k : 0<=i<4 => 0<=k<256 =>
+         ((lift_polyvec a).[i])%Vector.[k] = (lift_array1024 a).[256*i+k].
+move => ib lb; rewrite /lift_vector /lift_array1024 offunvE // mapiE 1:/# /=.
 by rewrite /lift_array256 /subarray256 mapiE //= initiE //=.
 qed.
 
 
 op unlift_polyvec(a : polyvec) = 
-   Array768.init (fun i => W16.of_int (as_sint (a.[i %/ 256])%Vector.[i%%256])).
+   Array1024.init (fun i => W16.of_int (as_sint (a.[i %/ 256])%Vector.[i%%256])).
 
 lemma vector_unlift a : 
     lift_polyvec (unlift_polyvec a) = a /\
-    signed_bound768_cxq (unlift_polyvec a) 0 768 1.
+    signed_bound1024_cxq (unlift_polyvec a) 0 1024 1.
 proof.
 split. 
 + rewrite /lift_vector /unlift_polyvec eq_vectorP => i ib.
@@ -51,42 +51,51 @@ split.
   rewrite !of_uintK /=; rewrite /as_sint qE /=.
   by smt(rg_asint asintK).
 
-rewrite /unlift_vector /signed_bound768_cxq => k kb; rewrite initiE //=.
+rewrite /unlift_vector /signed_bound1024_cxq => k kb; rewrite initiE //=.
 rewrite /to_sint /smod /= !of_uintK /= /as_sint qE /=.
 by smt(rg_asint).
 qed.
 
 
 lemma polyvec_csubq_corr_h ap :
-      hoare[Jkem768.M.__polyvec_csubq :
-           ap = lift_array768 r /\ pos_bound768_cxq r 0 768 2 
+      hoare[Jkem1024.M.__polyvec_csubq :
+           ap = lift_array1024 r /\ pos_bound1024_cxq r 0 1024 2 
            ==>
-           ap = lift_array768 res /\ pos_bound768_cxq res 0 768 1 ] . 
+           ap = lift_array1024 res /\ pos_bound1024_cxq res 0 1024 1 ] . 
 proof.
 proc.
 unroll for 2.
+wp;ecall (poly_csubq_corr_h (lift_array256 (Array256.init (fun i => r.[(3 * 256) + i])))).
 wp;ecall (poly_csubq_corr_h (lift_array256 (Array256.init (fun i => r.[(2 * 256) + i])))).
 wp;ecall (poly_csubq_corr_h (lift_array256 (Array256.init (fun i => r.[256 + i])))).
 wp;ecall (poly_csubq_corr_h (lift_array256 (Array256.init (fun i => r.[i])))).
 
 
 skip; move => &hr [#].
-rewrite /lift_array256 /pos_bound256_cxq /lift_array768 /pos_bound768_cxq /=.
+rewrite /lift_array256 /pos_bound256_cxq /lift_array1024 /pos_bound1024_cxq /=.
 
 move => -> bnd /=;split; 1: by move => *; rewrite initiE /#.
 
 move => bnd1 result [#] rval rbnd; rewrite tP in rval.
-split; 1: by move => *; rewrite !initiE //= !Array768.initiE /= /#.
+split; 1: by move => *; rewrite !initiE //= !Array1024.initiE /= /#.
 
 move => bnd2 resul2 [#] rva2 rbnd2; rewrite tP in rva2.
 rewrite !land_foo.
 split;1:by   move => *; do 3!(rewrite initiE /= 1:/#)  => /#.
 
 move => resul3 [#]  rva3 rbnd3; rewrite tP in rva3.
+rewrite !land_foo.
+split;1:by   move => *; do 4!(rewrite initiE /= 1:/#)  => /#.
+
+move => resul4 [#]  rva4 rbnd4; rewrite tP in rva4.
 
 split. 
 
 + rewrite tP => k kb; rewrite !mapiE 1,2:/# /=;  do 3!(rewrite initiE /= 1:/#).
+
+case (768 <= k && k < 1024).
++ move => kb0 /=;move : (rva4 (k - 768) _); 1: smt().
+  by rewrite !mapiE 1,2:/# //= !initiE 1:/# //= !initiE 1:/# //= !initiE //= !initiE //= /#. 
 
 case (512 <= k && k < 768).
 + move => kb0 /=;move : (rva3 (k - 512) _); 1: smt().
@@ -96,21 +105,21 @@ move => case1;case (256 <= k && k < 512).
 + move => kb0 /=;move : (rva2 (k - 256) _); 1: smt().
   by rewrite !mapiE 1,2:/# //= !initiE 1:/# //= !initiE //= /#.  
 
-move => case2;have : (0 <= k && k < 256); 1:smt().
+move => *;have : (0 <= k && k < 256); 1:smt().
 move => kb0 /=;move : (rval (k) kb0).
   by rewrite !mapiE 1,2:/# //= !initiE /#.
 
-by smt(Array768.initiE).
+by smt(Array1024.initiE).
 qed. 
 
-lemma polyvec_csubq_ll : islossless Jkem768.M.__polyvec_csubq 
-  by proc; unroll for 2;do 3! (wp;call poly_csubq_ll).
+lemma polyvec_csubq_ll : islossless Jkem1024.M.__polyvec_csubq 
+  by proc; unroll for 2;do 4! (wp;call poly_csubq_ll).
 
 lemma polyvec_csubq_corr ap :
-      phoare[Jkem768.M.__polyvec_csubq :
-           ap = lift_array768 r /\ pos_bound768_cxq r 0 768 2 
+      phoare[Jkem1024.M.__polyvec_csubq :
+           ap = lift_array1024 r /\ pos_bound1024_cxq r 0 1024 2 
            ==>
-           ap = lift_array768 res /\ pos_bound768_cxq res 0 768 1 ] = 1%r
+           ap = lift_array1024 res /\ pos_bound1024_cxq res 0 1024 1 ] = 1%r
   by conseq polyvec_csubq_ll (polyvec_csubq_corr_h ap). 
 
 lemma truncation1 x :
@@ -172,52 +181,52 @@ rewrite /truncateu8 /= !of_uintK /=.
 by rewrite !(modz_small _ 18446744073709551616); 1..3: smt().
 qed.
 
-lemma i_poly_compress_ll : islossless Jkem768.M._i_poly_compress.
+lemma i_poly_compress_ll : islossless Jkem1024.M._i_poly_compress.
 proc.
-while (0 <=  i <= 128) (128-i); last 
+while (0 <=  i <= 280) (280-i); last 
    by wp; call (poly_csubq_ll); auto =>  /> /#. 
-by auto => /#.
+by move => *; unroll for ^while;auto => /#.
 qed.
 
 
 (********** BEGIN BDEP PROOF OF COMPRESS  **************)
 require import Bindings.
 
-lemma i_polyvec_compress_ll : islossless Jkem768.M.__i_polyvec_compress.
+lemma i_polyvec_compress_ll : islossless Jkem1024.M.__i_polyvec_compress.
 proc.
-wp;while (0 <=  i <= 768) (768-i); last 
+wp;while (0 <=  i <= 1040) (1040-i); last 
    by wp; call (polyvec_csubq_ll); auto =>  /> /#. 
-by move => ?;unroll for ^while;auto => /> /#.
+by move => *;unroll for ^while;auto => /> /#.
 qed.
 
-op compress10_circuit(a : W16.t) : W10.t = 
+op compress11_circuit(a : W16.t) : W11.t = 
    if (a \ult W16.of_int 3329) then  
-   truncate64_10 (srl_64 ((sll_64 (zeroextu64 a) (W64.of_int 10) + W64.of_int 1665) * W64.of_int 1290167) (W64.of_int 32))
+   truncate64_11 (srl_64 ((sll_64 (zeroextu64 a) (W64.of_int 11) + W64.of_int 1664) * W64.of_int 645084) (W64.of_int 31))
    else 
-   truncate64_10 (srl_64 ((sll_64 (zeroextu64 (W16_sub a (W16.of_int 3329))) (W64.of_int 10) + W64.of_int 1665) * W64.of_int 1290167) (W64.of_int 32)).
+   truncate64_11 (srl_64 ((sll_64 (zeroextu64 (W16_sub a (W16.of_int 3329))) (W64.of_int 11) + W64.of_int 1664) * W64.of_int 645084) (W64.of_int 31)).
 
 module CompressInit = {
-    proc compressInit(rp: W8.t Array960.t, a: W16.t Array768.t) : W8.t Array960.t = {
-       rp <- init_960_8 (fun i => W8.zero);
-       rp <@ Jkem768.M.__i_polyvec_compress(rp,a);
+    proc compressInit(rp: W8.t Array1408.t, a: W16.t Array1024.t) : W8.t Array1408.t = {
+       rp <- init_1408_8 (fun i => W8.zero);
+       rp <@ Jkem1024.M.__i_polyvec_compress(rp,a);
        return rp;
     }
 }.
 
 lemma compressinit_ll : islossless CompressInit.compressInit.
 proc;inline 2.
-wp;while (0 <=  i <= 768) (768-i); last 
+wp;while (0 <=  i <= 1040) (1040-i); last 
    by wp; call (polyvec_csubq_ll); auto =>  /> /#. 
 by move => ?;unroll for ^while;auto => /> /#.
 qed.
 
 import BitEncoding BS2Int BitChunking.
 
-lemma output_pack_960_8(l : bool list) :
- size l = 960*8 =>
+lemma output_pack_1408_8(l : bool list) :
+ size l = 1408*8 =>
  flatten
   (map W8.w2bits
-     (to_list (Array960.of_list W8.zero (BitsToBytes l)))) = l.
+     (to_list (Array1408.of_list W8.zero (BitsToBytes l)))) = l.
 move => *.
 rewrite of_listK; 1: by rewrite size_BitsToBytes /#.
 have ? : size (flatten (map W8.w2bits (BitsToBytes l))) = size l.
@@ -234,57 +243,68 @@ rewrite -(nth_flatten _ 8);1: by rewrite allP => * /=;smt(in_chunk_size).
 by rewrite chunkK /#.
 qed.
 
-from JazzEC require import Array4.
+from JazzEC require import Array8.
 lemma i_polyvec_compress_corr_h _aw  : 
-    hoare [Jkem768.M.__i_polyvec_compress  :
-             pos_bound768_cxq a 0 768 2 /\
+    hoare [Jkem1024.M.__i_polyvec_compress  :
+             pos_bound1024_cxq a 0 1024 2 /\
              a = _aw
               ==>
-             res = encode10_vec (compress_polyvec 10 (lift_polyvec _aw)) 
+             res = encode11_vec (compress_polyvec 11 (lift_polyvec _aw)) 
              ].
 proof.
 bypr => &m H.
 rewrite Pr[mu_not].
 have -> : Pr[M.__i_polyvec_compress(rp{m}, a{m}) @ &m : true] = 1%r by byphoare => //;apply i_polyvec_compress_ll.
-have : Pr[M.__i_polyvec_compress(rp{m}, a{m}) @ &m : res = encode10_vec (compress_polyvec 10 (lift_polyvec _aw))  ] = 1%r; last by smt().
-have <- : Pr[ CompressInit.compressInit(rp{m}, a{m}) @ &m : res = encode10_vec (compress_polyvec 10 (lift_polyvec _aw)) ] = 1%r; last first.
+have : Pr[M.__i_polyvec_compress(rp{m}, a{m}) @ &m : res = encode11_vec (compress_polyvec 11 (lift_polyvec _aw))  ] = 1%r; last by smt().
+have <- : Pr[ CompressInit.compressInit(rp{m}, a{m}) @ &m : res = encode11_vec (compress_polyvec 11 (lift_polyvec _aw)) ] = 1%r; last first.
 + byequiv (: ={a} ==> ={res}) => //.
   proc;inline *.
   admit.
 
-byphoare (: pos_bound768_cxq a 0 768 2 /\  a = _aw ==> 
-   res = encode10_vec (compress_polyvec 10 (lift_polyvec _aw)))   => //.
+byphoare (: pos_bound1024_cxq a 0 1024 2 /\  a = _aw ==> 
+   res = encode11_vec (compress_polyvec 11 (lift_polyvec _aw)))   => //.
 conseq compressinit_ll (: _  ==> _);1:smt(). 
 proc; inline *.
 proc change ^while.1: (init_256_16 (fun i => r.[256*i0+i]));1: by auto.
 proc change ^while.^while.2: (W16_sub t0 (W16.of_int 3329)); 1: by auto.
 proc change ^while.^while.4 : (sra_16 b0 (W16.of_int 15)); 1: by auto.
-proc change ^while.5: (init_768_16 (fun (i_0 : int) => if 256 * i0 <= i_0 < 256 * i0 + 256 then aux.[i_0 - 256 * i0] else r.[i_0]));1: by auto.
-proc change ^while{2}.^while.2: (t.[k<-sll_64 t.[k] (W64.of_int 10)]); 1: by auto.
-proc change ^while{2}.^while.5: (t.[k<-srl_64 t.[k] (W64.of_int 32)]); 1: by auto.
-proc change ^while{2}.8:  (srl_16 b (W16.of_int 8)); 1: by auto.
-proc change ^while{2}.10:  (sll_16 c (W16.of_int 2)); 1: by auto.
-proc change ^while{2}.15:  (srl_16 b (W16.of_int 6)); 1: by auto.
-proc change ^while{2}.17:  (sll_16 c (W16.of_int 4)); 1: by auto.
-proc change ^while{2}.22:  (srl_16 b (W16.of_int 4)); 1: by auto.
-proc change ^while{2}.24:  (sll_16 c (W16.of_int 6)); 1: by auto.
-proc change ^while{2}.28: (t.[3<-srl_64 t.[3] (W64.of_int 2)]); 1: by auto.
+proc change ^while.5: (init_1024_16 (fun (i_0 : int) => if 256 * i0 <= i_0 < 256 * i0 + 256 then aux.[i_0 - 256 * i0] else r.[i_0]));1: by auto.
+proc change ^while{2}.^while.2: (sll_64 d0 (W64.of_int 11)); 1: by auto.
+proc change ^while{2}.^while.5: (srl_64 d0 (W64.of_int 31)); 1: by auto.
+proc change ^while{2}.7:  (srl_16 b (W16.of_int 8)); 1: by auto.
+proc change ^while{2}.9:  (sll_16 c (W16.of_int 3)); 1: by auto.
+proc change ^while{2}.14:  (srl_16 b (W16.of_int 5)); 1: by auto.
+proc change ^while{2}.16:  (sll_16 c (W16.of_int 6)); 1: by auto.
+proc change ^while{2}.21:  (srl_16 b (W16.of_int 2)); 1: by auto.
+proc change ^while{2}.25:  (srl_16 b (W16.of_int 10)); 1: by auto.
+proc change ^while{2}.27:  (sll_16 c (W16.of_int 1)); 1: by auto.
+proc change ^while{2}.32:  (srl_16 b (W16.of_int 7)); 1: by auto.
+proc change ^while{2}.34:  (sll_16 c (W16.of_int 4)); 1: by auto.
+proc change ^while{2}.39:  (srl_16 b (W16.of_int 4)); 1: by auto.
+proc change ^while{2}.41:  (sll_16 c (W16.of_int 7)); 1: by auto.
+proc change ^while{2}.46:  (srl_16 b (W16.of_int 1)); 1: by auto.
+proc change ^while{2}.50:  (srl_16 b (W16.of_int 9)); 1: by auto.
+proc change ^while{2}.52:  (sll_16 c (W16.of_int 2)); 1: by auto.
+proc change ^while{2}.57:  (srl_16 b (W16.of_int 6)); 1: by auto.
+proc change ^while{2}.59:  (sll_16 c (W16.of_int 5)); 1: by auto.
+proc change ^while{2}.63: (t.[7<-srl_16 t.[7] (W16.of_int 3)]); 1: by auto.
 
-unroll for 10.
-cfold ^i<-.
-do 196!(unroll for ^while).
+proc change 5 : (init_8_16(fun i => W16.zero));1:by admit.
+
+swap 6 5.
+unroll for 9.
+do 133!(unroll for ^while).
 cfold ^j<-.
 cfold ^i<-.
 cfold ^k<-.
 cfold ^i1<-.
 cfold ^i0<-.
 wp -6.
-proc change 5 : (init_4_64(fun i => W64.zero));1:by admit.
-bdep 16 10 [_aw] [a] [rp0] compress10_circuit pcond_reduced. 
+bdep 16 11 [_aw] [a] [rp0] compress11_circuit pcond_reduced. 
 
 (* BDEP pre conseq *)
 + move => &hr />; rewrite flatten1 /= pre_lane_commute_in_aligned 1:/# //=.
-  rewrite allP /pos_bound768_cxq /= => Hb. 
+  rewrite allP /pos_bound1024_cxq /= => Hb. 
   rewrite /pcond_reduced /= /tolist /= => x.
   rewrite  mkseqP => He;elim He => /= i [ib?]; rewrite ultE /=.
   have := Hb i; rewrite ib /= qE /=.
@@ -297,26 +317,26 @@ bdep 16 10 [_aw] [a] [rp0] compress10_circuit pcond_reduced.
 move => &hr [#]/= H0 <- rr; rewrite /= !flatten1.
 move => H1.
 
-apply (inj_eq Array960.to_list Array960.to_list_inj).
+apply (inj_eq Array1408.to_list Array1408.to_list_inj).
 apply (flatten_map_eq _ _ W8.w2bits 8 _ W8.w2bits_inj W8.size_w2bits);1:smt().
-have -> := post_lane_commute_in_aligned (to_list a{hr}) (to_list rr) W16.w2bits W16.bits2w W8.w2bits W8.bits2w W10.w2bits W10.bits2w  compress10_circuit 16 10 8 _ _ _ _ _ _ _ _ _ _ _ _ H1;1..12:
-    smt(Array960.size_to_list Array768.size_to_list W16.bits2wK BVA_Top_Bindings_W10_t.oflistP).
+have -> := post_lane_commute_in_aligned (to_list a{hr}) (to_list rr) W16.w2bits W16.bits2w W8.w2bits W8.bits2w W11.w2bits W11.bits2w  compress11_circuit 16 11 8 _ _ _ _ _ _ _ _ _ _ _ _ H1;1..12:
+    smt(Array1408.size_to_list Array1024.size_to_list W16.bits2wK BVA_Top_Bindings_W11_t.oflistP).
 
-rewrite output_pack_960_8. 
-+ rewrite (EclibExtra.size_flatten' 10);1: smt(mapP BS2Int.size_int2bs).
+rewrite output_pack_1408_8. 
++ rewrite (EclibExtra.size_flatten' 11);1: smt(mapP BS2Int.size_int2bs).
   by rewrite size_map size_to_list /=.
 
 congr.
-rewrite /compress10_circuit /compress_polyvec /fromarray256  -map_comp -map_comp -map_comp /(\o) /=.  
+rewrite /compress11_circuit /compress_polyvec /fromarray256  -map_comp -map_comp -map_comp /(\o) /=.  
 apply (eq_from_nth witness); 1: by rewrite !size_map //.
 rewrite size_map size_iota /max /= => i ib; rewrite !(nth_map witness) //=;1,2:smt(size_iota).
 rewrite nth_iota 1:/# mapiE 1:/# initiE 1:/# /= /lift_polyvec /=.
 case (0<=i<256).
 + move => ? /=.
-  rewrite  !getvE offunvE 1:/# /= -(BVA_Top_Bindings_W10_t.oflistP (int2bs 10 (compress 10 (lift_array256 (subarray256 a{hr} 0)).[i]))); 1: by rewrite BS2Int.size_int2bs /#.
-congr; rewrite -BVA_Top_Bindings_W10_t.ofintP /lift_array256 /subarray256 !mapiE 1:/# /= initiE 1:/# /=. 
+  rewrite  !getvE offunvE 1:/# /= -(BVA_Top_Bindings_W11_t.oflistP (int2bs 11 (compress 11 (lift_array256 (subarray256 a{hr} 0)).[i]))); 1: by rewrite BS2Int.size_int2bs /#.
+congr; rewrite -BVA_Top_Bindings_W11_t.ofintP /lift_array256 /subarray256 !mapiE 1:/# /= initiE 1:/# /=. 
 
-rewrite /truncate64_10 to_uint_eq.
+rewrite /truncate64_11 to_uint_eq.
 (* This is now the equivalence betwen specs. It's made slightly more verbose
    because the impl circuit is only proved correct wrt compress for values
    in the q range. *)
@@ -324,7 +344,7 @@ rewrite ultE /=.
 case (to_uint a{hr}.[i] < 3329) => /= *.
 + rewrite -Fq.compress_impl_large //=; 1: by rewrite /bpos16 qE /= /to_sint /smod /=;smt(W16.to_uint_cmp).     
   rewrite /srl_64 /sll_64 /(`<<`) /(`>>`) !of_uintK /= /#. 
-have := H0;rewrite /pos_bound768_cxq qE /= => H00.
+have := H0;rewrite /pos_bound1024_cxq qE /= => H00.
 
 have ? : 0 <= to_sint ((W16_sub a{hr}.[i] (W16.of_int 3329))) < 3329.
 +  rewrite /bpos16 to_sintB_small /=;1: by rewrite  /(to_sint (W16.of_int 3329))  W16.of_uintK /= /smod /=;smt(size_map size_iota). 
@@ -341,10 +361,10 @@ by rewrite /srl_64 /sll_64 /(`<<`) /(`>>`) !of_uintK /= /#.
 
 case (256<=i<512).
 + move => ?? /=.
-  rewrite  !getvE offunvE 1:/# /= -(BVA_Top_Bindings_W10_t.oflistP (int2bs 10 (compress 10 (lift_array256 (subarray256 a{hr} 1)).[i-256]))); 1: by rewrite BS2Int.size_int2bs /#.
-congr; rewrite -BVA_Top_Bindings_W10_t.ofintP /lift_array256 /subarray256 !mapiE 1:/# /= initiE 1:/# /=. 
+  rewrite  !getvE offunvE 1:/# /= -(BVA_Top_Bindings_W11_t.oflistP (int2bs 11 (compress 11 (lift_array256 (subarray256 a{hr} 1)).[i-256]))); 1: by rewrite BS2Int.size_int2bs /#.
+congr; rewrite -BVA_Top_Bindings_W11_t.ofintP /lift_array256 /subarray256 !mapiE 1:/# /= initiE 1:/# /=. 
 
-rewrite /truncate64_10 to_uint_eq.
+rewrite /truncate64_11 to_uint_eq.
 (* This is now the equivalence betwen specs. It's made slightly more verbose
    because the impl circuit is only proved correct wrt compress for values
    in the q range. *)
@@ -352,7 +372,7 @@ rewrite ultE /=.
 case (to_uint a{hr}.[i] < 3329) => /= *.
 + rewrite -Fq.compress_impl_large //=; 1: by rewrite /bpos16 qE /= /to_sint /smod /=;smt(W16.to_uint_cmp).     
   rewrite /srl_64 /sll_64 /(`<<`) /(`>>`) !of_uintK /= /#. 
-have := H0;rewrite /pos_bound768_cxq qE /= => H00.
+have := H0;rewrite /pos_bound1024_cxq qE /= => H00.
 
 have ? : 0 <= to_sint ((W16_sub a{hr}.[i] (W16.of_int 3329))) < 3329.
 +  rewrite /bpos16 to_sintB_small /=;1: by rewrite  /(to_sint (W16.of_int 3329))  W16.of_uintK /= /smod /=;smt(size_map size_iota). 
@@ -367,9 +387,37 @@ have -> : (incoeff (to_sint a{hr}.[i])) = (incoeff (to_sint (W16_sub a{hr}.[i] (
 rewrite -Fq.compress_impl_large //=;1:by smt().
 by rewrite /srl_64 /sll_64 /(`<<`) /(`>>`) !of_uintK /= /#. 
 
- move => ?? /=.
-  rewrite  !getvE offunvE 1:/# /= -(BVA_Top_Bindings_W10_t.oflistP (int2bs 10 (compress 10 (lift_array256 (subarray256 a{hr} 2)).[i-512]))); 1: by rewrite BS2Int.size_int2bs /#.
-congr; rewrite -BVA_Top_Bindings_W10_t.ofintP /lift_array256 /subarray256 !mapiE 1:/# /= initiE 1:/# /=. 
+case (512<=i<768).
++ move => ??? /=.
+  rewrite  !getvE offunvE 1:/# /= -(BVA_Top_Bindings_W11_t.oflistP (int2bs 11 (compress 11 (lift_array256 (subarray256 a{hr} 2)).[i-512]))); 1: by rewrite BS2Int.size_int2bs /#.
+congr; rewrite -BVA_Top_Bindings_W11_t.ofintP /lift_array256 /subarray256 !mapiE 1:/# /= initiE 1:/# /=. 
+
+rewrite /truncate64_11 to_uint_eq.
+(* This is now the equivalence betwen specs. It's made slightly more verbose
+   because the impl circuit is only proved correct wrt compress for values
+   in the q range. *)
+rewrite ultE /=. 
+case (to_uint a{hr}.[i] < 3329) => /= *.
++ rewrite -Fq.compress_impl_large //=; 1: by rewrite /bpos16 qE /= /to_sint /smod /=;smt(W16.to_uint_cmp).     
+  rewrite /srl_64 /sll_64 /(`<<`) /(`>>`) !of_uintK /= /#. 
+have := H0;rewrite /pos_bound1024_cxq qE /= => H00.
+
+have ? : 0 <= to_sint ((W16_sub a{hr}.[i] (W16.of_int 3329))) < 3329.
++  rewrite /bpos16 to_sintB_small /=;1: by rewrite  /(to_sint (W16.of_int 3329))  W16.of_uintK /= /smod /=;smt(size_map size_iota). 
+   by rewrite  /(to_sint (W16.of_int 3329))  W16.of_uintK /= /smod /=; smt(size_map size_iota W16.to_uint_cmp).
+
+have ? : to_sint ((W16_sub a{hr}.[i] (W16.of_int 3329))) = to_sint a{hr}.[i] -  3329.
++  rewrite to_sintB_small /=;1: by rewrite  /(to_sint (W16.of_int 3329))  W16.of_uintK /= /smod /=;smt(size_map size_iota). 
+   by rewrite  /(to_sint (W16.of_int 3329))  W16.of_uintK /= /smod /=; smt(size_map size_iota W16.to_uint_cmp).
+
+have -> : (incoeff (to_sint a{hr}.[i])) = (incoeff (to_sint (W16_sub a{hr}.[i] (W16.of_int 3329)))) by  rewrite -eq_incoeff;  smt().  
+
+rewrite -Fq.compress_impl_large //=;1:by smt().
+by rewrite /srl_64 /sll_64 /(`<<`) /(`>>`) !of_uintK /= /#. 
+
+ move => ??? /=.
+  rewrite  !getvE offunvE 1:/# /= -(BVA_Top_Bindings_W11_t.oflistP (int2bs 11 (compress 11 (lift_array256 (subarray256 a{hr} 3)).[i-768]))); 1: by rewrite BS2Int.size_int2bs /#.
+congr; rewrite -BVA_Top_Bindings_W11_t.ofintP /lift_array256 /subarray256 !mapiE 1:/# /= initiE 1:/# /=. 
 
 rewrite /truncate64_10 to_uint_eq.
 (* This is now the equivalence betwen specs. It's made slightly more verbose
@@ -379,7 +427,7 @@ rewrite ultE /=.
 case (to_uint a{hr}.[i] < 3329) => /= *.
 + rewrite -Fq.compress_impl_large //=; 1: by rewrite /bpos16 qE /= /to_sint /smod /=;smt(W16.to_uint_cmp).     
   rewrite /srl_64 /sll_64 /(`<<`) /(`>>`) !of_uintK /= /#. 
-have := H0;rewrite /pos_bound768_cxq qE /= => H00.
+have := H0;rewrite /pos_bound1024_cxq qE /= => H00.
 
 have ? : 0 <= to_sint ((W16_sub a{hr}.[i] (W16.of_int 3329))) < 3329.
 +  rewrite /bpos16 to_sintB_small /=;1: by rewrite  /(to_sint (W16.of_int 3329))  W16.of_uintK /= /smod /=;smt(size_map size_iota). 
@@ -400,125 +448,140 @@ qed.
 
 
 lemma i_polyvec_compress_corr _aw :
-    phoare [Jkem768.M.__i_polyvec_compress  :
-pos_bound768_cxq a 0 768 2 /\
+    phoare [Jkem1024.M.__i_polyvec_compress  :
+pos_bound1024_cxq a 0 1024 2 /\
              a = _aw
               ==>
-             res = encode10_vec (compress_polyvec 10 (lift_polyvec _aw)) 
+             res = encode11_vec (compress_polyvec 11 (lift_polyvec _aw)) 
               ] = 1%r
   by conseq i_polyvec_compress_ll (i_polyvec_compress_corr_h _aw).
 
 lemma polyvec_add_corr_h _a _b ab bb :
       0 <= ab <= 6 => 0 <= bb <= 3 =>
-      hoare[Jkem768.M.__polyvec_add2 :
-           _a = lift_array768 r /\
-           _b = lift_array768 b /\
-           signed_bound768_cxq r 0 768 ab /\
-           signed_bound768_cxq b 0 768 bb 
+      hoare[Jkem1024.M.__polyvec_add2 :
+           _a = lift_array1024 r /\
+           _b = lift_array1024 b /\
+           signed_bound1024_cxq r 0 1024 ab /\
+           signed_bound1024_cxq b 0 1024 bb 
            ==>
-           signed_bound768_cxq res 0 768 (ab + bb) /\ 
-           forall k, 0 <= k < 768 =>
+           signed_bound1024_cxq res 0 1024 (ab + bb) /\ 
+           forall k, 0 <= k < 1024 =>
               incoeff (to_sint res.[k]) = _a.[k] + _b.[k]]. 
 proof.
 move => abb bbb;  move : (poly_add_corr_impl_h ab bb abb bbb) => H.
 proc.
 unroll for 2.
+wp;ecall (H (lift_array256 (Array256.init (fun i => r.[(3 * 256) + i]))) (lift_array256 (Array256.init (fun i => b.[(3 * 256) + i])))).
 wp;ecall (H (lift_array256 (Array256.init (fun i => r.[(2 * 256) + i]))) (lift_array256 (Array256.init (fun i => b.[(2 * 256) + i])))).
 wp;ecall (H (lift_array256 (Array256.init (fun i => r.[256 + i]))) (lift_array256 (Array256.init (fun i => b.[256 + i])))).
 wp;ecall (H (lift_array256 (Array256.init (fun i => r.[i]))) (lift_array256 (Array256.init (fun i => b.[i])))).
 clear H.
 skip => &hr.
-rewrite /signed_bound768_cxq /signed_bound_cxq /lift_array768 /lift_array256 /=.
+rewrite /signed_bound1024_cxq /signed_bound_cxq /lift_array1024 /lift_array256 /=.
 move => [#] ->-> 2?.
 do split; 1..2: by move => *; rewrite !initiE //= /#.
 move => [#] H H0 ?? res1 [#] resb1 resv1.
 do split.
-+ by move => k kb; move : (resb1 k kb); rewrite !initiE  //= !Array768.initiE  /#.
++ by move => k kb; move : (resb1 k kb); rewrite !initiE  //= !Array1024.initiE  /#.
 + by move => k kb; move : (resb1 k kb); rewrite !initiE  //= /#.
 
 move => [#]  vsofar bsofar ?? res2 [#] res2b res2v.
 rewrite !land_foo.
 do split.
-+ move => k kb; rewrite !initiE  /=1:/# !Array768.initiE  /= 1:/#.
++ move => k kb; rewrite !initiE  /=1:/# !Array1024.initiE  /= 1:/#.
   rewrite  (_: (256 <= 512 + k && 512 + k < 512)=false) /= 1:/#.
-  by rewrite !Array768.initiE  /= /#.
+  by rewrite !Array1024.initiE  /= /#.
 + by move => k kb;rewrite !initiE  /= /#.
 
 move => [#]  res3 [#] res3b res3v.
+rewrite !land_foo.
 do split.
-+ move => k kb; rewrite !initiE  /= 1:/# !Array768.initiE  /= 1:/#.
-  case (512 <= k && k < 768); 1: by smt().
-  case (256 <= k && k < 512); 1: by smt().
-  by move => *; rewrite !initiE /= /#.
++ move => k kb; rewrite !initiE  /= 1:/# !Array1024.initiE  /= 1:/#. 
+  rewrite  (_: (512 <= 768 + k && 768 + k < 768)=false) /= 1:/#.
+  by rewrite !Array1024.initiE  /= 1:/# /= !Array1024.initiE  /= /#.
++ by move => k kb;rewrite !initiE  /# /=. 
 
-move => k [#] kbl kbh; rewrite !initiE  //= !Array768.initiE  /= 1:/# !mapiE //= !initiE //=.
+move => [#]  res4 [#] res4b res4v.
+do split.
++ move => k kb; rewrite !initiE  /= 1:/# !Array1024.initiE  /= 1:/#;  smt(Array1024.initiE).
+
+
+move => k [#] kbl kbh; rewrite !initiE  //= !Array1024.initiE  /= 1:/# !mapiE //= !initiE //=.
+case (768 <= k && k < 1024).
++ move => kbb.
+  rewrite (res4v (k - 768) _) 1:/# !mapiE /= 1..2:/# !initiE /= 1..2:/#.
+  by rewrite !Array1024.initiE /= 1:/# !Array1024.initiE /= 1:/# !Array1024.initiE /= /#.
+
 case (512 <= k && k < 768).
 + move => kbb.
   rewrite (res3v (k - 512) _) 1:/# !mapiE /= 1..2:/# !initiE /= 1..2:/#.
-  by rewrite !Array768.initiE /= 1:/# !Array768.initiE /= /#.
+  by rewrite !Array1024.initiE /= 1:/# !Array1024.initiE /= /#.
 
 move => nkbb.
 case (256 <= k && k < 512).
 + move => kbb.
   rewrite (res2v (k - 256) _) 1:/# !mapiE /= 1..2:/# !initiE /= 1..2:/#.
-  by rewrite !Array768.initiE /= /#.
+  by rewrite !Array1024.initiE /= /#.
 
-move => nkbb2.
+move => *.
+rewrite initiE 1:/# /=. 
 have -> : 0 <= k < 256 by smt().
 by rewrite (resv1 k _) 1:/# !mapiE /= 1..2:/# !initiE /= 1..2:/#.
 qed.
 
-lemma polyvec_add_ll  : islossless Jkem768.M.__polyvec_add2 by proc; unroll for 2;do 3! (wp; call poly_add_ll).
+lemma polyvec_add_ll  : islossless Jkem1024.M.__polyvec_add2 by proc; unroll for 2;do 4! (wp; call poly_add_ll).
 
 lemma polyvec_add_corr  _a _b ab bb:
     0 <= ab <= 6 => 0 <= bb <= 3 =>
-   phoare[Jkem768.M.__polyvec_add2 :
-           _a = lift_array768 r /\
-           _b = lift_array768 b /\
-           signed_bound768_cxq r 0 768 ab /\
-           signed_bound768_cxq b 0 768 bb 
+   phoare[Jkem1024.M.__polyvec_add2 :
+           _a = lift_array1024 r /\
+           _b = lift_array1024 b /\
+           signed_bound1024_cxq r 0 1024 ab /\
+           signed_bound1024_cxq b 0 1024 bb 
            ==>
-           signed_bound768_cxq res 0 768 (ab + bb) /\ 
-           forall k, 0 <= k < 768 =>
+           signed_bound1024_cxq res 0 1024 (ab + bb) /\ 
+           forall k, 0 <= k < 1024 =>
               incoeff (to_sint res.[k]) = _a.[k] + _b.[k] ]  = 1%r by 
   move => abb bbb; conseq polyvec_add_ll (polyvec_add_corr_h  _a _b ab bb abb bbb).
 
 lemma polyvec_add_corr_impl  ab bb:
     0 <= ab <= 6 => 0 <= bb <= 3 =>
     forall _a _b,
-   phoare[Jkem768.M.__polyvec_add2 :
-           _a = lift_array768 r /\
-           _b = lift_array768 b /\
-           signed_bound768_cxq r 0 768 ab /\
-           signed_bound768_cxq b 0 768 bb 
+   phoare[Jkem1024.M.__polyvec_add2 :
+           _a = lift_array1024 r /\
+           _b = lift_array1024 b /\
+           signed_bound1024_cxq r 0 1024 ab /\
+           signed_bound1024_cxq b 0 1024 bb 
            ==>
-           signed_bound768_cxq res 0 768 (ab + bb) /\ 
-           forall k, 0 <= k < 768 =>
+           signed_bound1024_cxq res 0 1024 (ab + bb) /\ 
+           forall k, 0 <= k < 1024 =>
               incoeff (to_sint res.[k]) = _a.[k] + _b.[k] ]  = 1%r
   by move => abb bbb _a _b;  apply (polyvec_add_corr  _a _b ab bb abb bbb).
 
 (******************************************************)
 
 lemma polyvec_reduce_corr_h _a :
-      hoare[Jkem768.M.__polyvec_reduce :
-          _a = lift_array768 r ==> 
-          _a = lift_array768 res /\
-          forall k, 0 <= k < 768 => bpos16 res.[k] (2*q)].
+      hoare[Jkem1024.M.__polyvec_reduce :
+          _a = lift_array1024 r ==> 
+          _a = lift_array1024 res /\
+          forall k, 0 <= k < 1024 => bpos16 res.[k] (2*q)].
 proof.
 proc. 
 unroll for 2.
+wp;ecall (poly_reduce_corr_h (lift_array256 (Array256.init (fun i => r.[(3 * 256) + i])))).
 wp;ecall (poly_reduce_corr_h (lift_array256 (Array256.init (fun i => r.[(2 * 256) + i])))).
 wp;ecall (poly_reduce_corr_h (lift_array256 (Array256.init (fun i => r.[256 + i])))).
 wp;ecall (poly_reduce_corr_h (lift_array256 (Array256.init (fun i => r.[i])))).
   
-skip=>  &hr; rewrite /lift_array256 /lift_array768 => ->.
+skip=>  &hr; rewrite /lift_array256 /lift_array1024 => ->.
 rewrite !land_foo; split => /=.
 
-+ rewrite tP => k kb; rewrite !mapiE //= !initiE //= !Array768.initiE  /=.
++ rewrite tP => k kb; rewrite !mapiE //= !initiE //= !Array1024.initiE  /=.
 
 
-move => res1 [#] res1v res1b res2 [#] res2v res2b res3 [#]  res3v res3b.
+move => res1 [#] res1v res1b res2 [#] res2v res2b res3 [#]  res3v res3b res4 [#]  res4v res4b.
 
+rewrite tP in res4v.
 rewrite tP in res3v.
 rewrite tP in res2v.
 rewrite tP in res1v.
@@ -529,33 +592,38 @@ split.
   case (256 <= k && k < 512).
   + move => kbb.
     move : (res2v (k - 256) _); 1:smt(); rewrite !mapiE /= 1..4:/# !initiE /= 1..2:/#.
-    by rewrite !Array768.initiE  /=  /#. 
+     rewrite !Array1024.initiE  /=  1,2:/#  !Array1024.initiE  /=  /#. 
 
   move =>  nkbb2.
-  rewrite !mapiE 1..2:/# !Array768.initiE  /=  1:/#.
+  rewrite !mapiE 1..2:/# !Array1024.initiE  /=  1:/#.
 
   case (512 <= k && k < 768).
   + move => kbb.
-  move : (res3v (k-512) _); 1:smt(); rewrite !mapiE /= 1,2:/# !initiE /= 1:/# !initiE /= 1:/# !initiE /= /#.
+  move : (res3v (k-512) _); 1:smt(); rewrite !mapiE /= 1,2:/# !initiE /= 1,2:/# !initiE /= 1:/# !initiE /= /#.
 
-move => nkbb3.
-rewrite !Array768.initiE  /=  1:/#.
-rewrite !Array768.initiE  /=  1:/#.
-  move : (res1v (k) _); 1:smt(); rewrite !mapiE /= 1..2:/# !initiE /= 1:/# /#.
+  case (768 <= k && k < 1024).
+  + move => kbb.
+  move : (res4v (k-768) _); 1:smt().
+   rewrite !mapiE /= 1,2:/# !initiE /= 1:/# !initiE /= 1:/#  !initiE /= 1:/# !initiE /= /#.
 
-smt(Array768.initiE).
+move => *.
+rewrite !Array1024.initiE  /=  1:/#.
+rewrite !Array1024.initiE  /=  1:/#.
+  move : (res1v (k) _); 1:smt(); rewrite !mapiE /= 1,2:/# !initiE /#.
+
+smt(Array1024.initiE).
 
 qed.
 
 
 (* TODO *)
-lemma polyvec_reduce_ll: islossless Jkem768.M.__polyvec_reduce  by proc; unroll for 2;do 3! (wp; call poly_reduce_ll).
+lemma polyvec_reduce_ll: islossless Jkem1024.M.__polyvec_reduce  by proc; unroll for 2;do 4! (wp; call poly_reduce_ll).
 
 lemma polyvec_reduce_corr  _a :
-      phoare[Jkem768.M.__polyvec_reduce :
-          _a = lift_array768 r ==> 
-          _a = lift_array768 res /\
-          forall k, 0 <= k < 768 => bpos16 res.[k] (2*q)]  = 1%r 
+      phoare[Jkem1024.M.__polyvec_reduce :
+          _a = lift_array1024 r ==> 
+          _a = lift_array1024 res /\
+          forall k, 0 <= k < 1024 => bpos16 res.[k] (2*q)]  = 1%r 
 by conseq polyvec_reduce_ll (polyvec_reduce_corr_h  _a).
 
 (******************************************************)
@@ -671,86 +739,104 @@ qed.
 
 (********** BEGIN BDEP PROOF OF DECOMPRESS **************)
 
-op decompress10_circuit(c : W10.t) : W16.t = 
-  truncateu16 (srl_32 (((zeroextu10_32 c) * W32.of_int 3329) + W32.of_int 512) (W32.of_int 10)).
+op decompress11_circuit(c : W11.t) : W16.t = 
+  truncateu16 (srl_32 (((zeroextu11_32 c) * W32.of_int 3329) + W32.of_int 1024) (W32.of_int 11)).
 
-op pcond_true10(_: W10.t) = true.
+op pcond_true11(_: W11.t) = true.
 
 module DecompressInit = {
-    proc decompressInit(rp :  W16.t Array768.t, ap: W8.t Array960.t) : W16.t Array768.t = {
-       rp <- init_768_16 (fun i => W16.zero);
-       rp <@ Jkem768.M.__i_polyvec_decompress(rp,ap);
+    proc decompressInit(rp :  W16.t Array1024.t, ap: W8.t Array1408.t) : W16.t Array1024.t = {
+       rp <- init_1024_16 (fun i => W16.zero);
+       rp <@ Jkem1024.M.__i_polyvec_decompress(rp,ap);
        return rp;
     }
 }.
 
-lemma polyvec_decompress_ll : islossless Jkem768.M.__i_polyvec_decompress.
+lemma polyvec_decompress_ll : islossless Jkem1024.M.__i_polyvec_decompress.
  proc; inline *;wp. 
-  while (0 <= i <= 960) (960-i); last by  auto =>  /> /#.
-move => *;unroll for ^while;unroll for ^while;auto => /> /#.
+  while (0 <= i <= 1408) (1408-i); last by  auto =>  /> /#.
+move => *;auto => /> /#.
 qed.
 
 lemma decompressinit_ll : islossless DecompressInit.decompressInit.
  proc; inline *;wp. 
-  while (0 <= i <= 960) (960-i); last by  auto =>  /> /#.
-move => *;unroll for ^while;unroll for ^while;auto => /> /#.
+  while (0 <= i <= 1408) (1408-i); last by  auto =>  /> /#.
+move => *;auto => /> /#.
 qed.
 
-lemma polyvec_decompress_corr_h (_aw : W8.t Array960.t): 
-    hoare [Jkem768.M.__i_polyvec_decompress  :
+lemma polyvec_decompress_corr_h (_aw : W8.t Array1408.t): 
+    hoare [Jkem1024.M.__i_polyvec_decompress  :
              ap = _aw
               ==>
-             pos_bound768_cxq res 0 768 1 /\
-             lift_polyvec res = decompress_polyvec 10 (decode10_vec _aw) ].
+             pos_bound1024_cxq res 0 1024 1 /\
+             lift_polyvec res = decompress_polyvec 11 (decode11_vec _aw) ].
 bypr => &m H.
 rewrite Pr[mu_not].
 have -> : Pr[M.__i_polyvec_decompress(rp{m}, ap{m}) @ &m : true] = 1%r by byphoare => //;apply polyvec_decompress_ll.
-have : Pr[M.__i_polyvec_decompress(rp{m}, ap{m}) @ &m :pos_bound768_cxq res 0 768 1 /\
-             lift_polyvec res = decompress_polyvec 10 (decode10_vec _aw)] = 1%r; last by smt().
-have <- : Pr[ DecompressInit.decompressInit(rp{m}, ap{m}) @ &m : pos_bound768_cxq res 0 768 1 /\
-             lift_polyvec res = decompress_polyvec 10 (decode10_vec _aw)] = 1%r; last first.
+have : Pr[M.__i_polyvec_decompress(rp{m}, ap{m}) @ &m :pos_bound1024_cxq res 0 1024 1 /\
+             lift_polyvec res = decompress_polyvec 11 (decode11_vec _aw)] = 1%r; last by smt().
+have <- : Pr[ DecompressInit.decompressInit(rp{m}, ap{m}) @ &m : pos_bound1024_cxq res 0 1024 1 /\
+             lift_polyvec res = decompress_polyvec 11 (decode11_vec _aw)] = 1%r; last first.
 + byequiv (: arg{1}.`2 = arg{2}.`2 ==> ={res}) => //.
   proc;inline *.
   admit.
 
 byphoare (: ap = _aw ==> 
-   pos_bound768_cxq res 0 768 1 /\
-             lift_polyvec res = decompress_polyvec 10 (decode10_vec _aw)) => //.
+   pos_bound1024_cxq res 0 1024 1 /\
+             lift_polyvec res = decompress_polyvec 11 (decode11_vec _aw)) => //.
 conseq decompressinit_ll (: _  ==> _);1:smt(). 
 proc; inline *.
-proc change ^while.4: (t.[1<-srl_32 t.[1] (W32.of_int 2)]); 1: by auto.
-proc change ^while.6: (sll_32 d (W32.of_int 8));1: by auto.
-proc change ^while.9: (t.[2<-srl_32 t.[2] (W32.of_int 4)]); 1: by auto.
-proc change ^while.11: (sll_32 d (W32.of_int 6));1: by auto.
-proc change ^while.14: (t.[3<-srl_32 t.[3] (W32.of_int 6)]); 1: by auto.
-proc change ^while.16: (sll_32 d (W32.of_int 4));1: by auto.
-proc change ^while.19: (sll_32 d (W32.of_int 2));1: by auto.
-proc change ^while.^while{2}.3: (t.[k<-srl_32 t.[k] (W32.of_int 10)]);1: by auto.
-swap 5 1.
+proc change ^while.6: (sll_32 d1 (W32.of_int 8));1: by auto.
+proc change ^while.11: (srl_32 t0 (W32.of_int 11)); 1: by auto.
+proc change ^while.16: (srl_32 d0 (W32.of_int 3));1: by auto.
+proc change ^while.18: (sll_32 d1 (W32.of_int 5)); 1: by auto.
+proc change ^while.23: (srl_32 d0 (W32.of_int 11));1: by auto.
+proc change ^while.29: (srl_32 t0 (W32.of_int 6));1: by auto.
+proc change ^while.31: (sll_32 d0 (W32.of_int 2));1: by auto.
+proc change ^while.33: (sll_32 d1 (W32.of_int 10));1: by auto.
+proc change ^while.39: (srl_32 d0 (W32.of_int 11));1: by auto.
+proc change ^while.44: (srl_32 d0 (W32.of_int 1));1: by auto.
+proc change ^while.46: (sll_32 d1 (W32.of_int 7));1: by auto.
+proc change ^while.51: (srl_32 d0 (W32.of_int 11));1: by auto.
+proc change ^while.56: (srl_32 d0 (W32.of_int 4));1: by auto.
+proc change ^while.58: (sll_32 d1 (W32.of_int 4));1: by auto.
+proc change ^while.63: (srl_32 d0 (W32.of_int 11));1: by auto.
+proc change ^while.69: (srl_32 t1 (W32.of_int 7));1: by auto.
+proc change ^while.71: (sll_32 d0 (W32.of_int 1));1: by auto.
+proc change ^while.73: (sll_32 d1 (W32.of_int 9));1: by auto.
+proc change ^while.79: (srl_32 d0 (W32.of_int 11));1: by auto.
+proc change ^while.84: (srl_32 d0 (W32.of_int 2));1: by auto.
+proc change ^while.86: (sll_32 d1 (W32.of_int 6));1: by auto.
+proc change ^while.79: (srl_32 d0 (W32.of_int 11));1: by auto.
+proc change ^while.91: (srl_32 d0 (W32.of_int 11));1: by auto.
+proc change ^while.96: (srl_32 d0 (W32.of_int 5));1: by auto.
+proc change ^while.98: (sll_32 d1 (W32.of_int 3));1: by auto.
+proc change ^while.103: (srl_32 d0 (W32.of_int 11));1: by auto.
+
+swap 4 1.
 unroll for ^while.
-do 384!(unroll for ^while).
+cfold ^i<-.
 cfold ^j<-.
-cfold ^k<-.
-wp -4.
-proc change 4: (init_5_32 (fun _ => W32.zero));1: by admit.
-bdep 10 16 [_aw] [ap] [rp0] decompress10_circuit pcond_true10. 
+wp -3.
+bdep 11 16 [_aw] [ap] [rp0] decompress11_circuit pcond_true11. 
 
 (* BDEP pre conseq *)
-+ by move => &hr />; rewrite allP /pcond_true10 /=. 
++ by move => &hr />; rewrite allP /pcond_true11 /=. 
 
 (* BDEP post conseq *)
 
 (* We start with some boilerplate *)
 move => &hr [#]/= <- rr; rewrite /= !flatten1.
-move => H1; have H2 := post_lane_commute_out_aligned (to_list ap{hr}) (to_list rr) W8.w2bits W8.bits2w W10.w2bits W10.bits2w W16.w2bits W16.bits2w  decompress10_circuit 8 10 16 _ _ _ _ _ _ _ _ _ _ _ _ H1;1..12:
-smt(Array960.size_to_list Array768.size_to_list W16.bits2wK BVA_Top_Bindings_W10_t.oflistP).
+move => H1; have H2 := post_lane_commute_out_aligned (to_list ap{hr}) (to_list rr) W8.w2bits W8.bits2w W11.w2bits W11.bits2w W16.w2bits W16.bits2w  decompress11_circuit 8 11 16 _ _ _ _ _ _ _ _ _ _ _ _ H1;1..12:
+smt(Array1408.size_to_list Array1024.size_to_list W16.bits2wK BVA_Top_Bindings_W11_t.oflistP).
 
 have H3 : 
-   map decompress10_circuit (map W10.bits2w (chunk 10 (flatten (map W8.w2bits (to_list ap{hr}))))) =
-   map (W16.of_int \o asint) (to_list (decompress_polyvec 10 (decode10_vec ap{hr})).[0] ++ 
-                              to_list (decompress_polyvec 10 (decode10_vec ap{hr})).[1] ++ 
-                              to_list (decompress_polyvec 10 (decode10_vec ap{hr})).[2])%Vector.
-+ rewrite /decode10_vec /decompress_polyvec !map_cat !setvE !offunvE 1..3:/# /= !offunvK /vclamp /kvec /= /subarray256 /=.
+   map decompress11_circuit (map W11.bits2w (chunk 11 (flatten (map W8.w2bits (to_list ap{hr}))))) =
+   map (W16.of_int \o asint) (to_list (decompress_polyvec 11 (decode11_vec ap{hr})).[0] ++ 
+                              to_list (decompress_polyvec 11 (decode11_vec ap{hr})).[1] ++ 
+                              to_list (decompress_polyvec 11 (decode11_vec ap{hr})).[2] ++ 
+                              to_list (decompress_polyvec 11 (decode11_vec ap{hr})).[3])%Vector.
++ rewrite /decode11_vec /decompress_polyvec !map_cat !setvE !offunvE 1..4:/# /= !offunvK /vclamp /kvec /= /subarray256 /=.
   apply (eq_from_nth witness).
   + rewrite !size_map !size_cat !size_map !size_iota /max /=.
      rewrite (EclibExtra.size_flatten' 8);1:smt(mapP W8.size_w2bits). 
@@ -761,7 +847,7 @@ have H3 :
    rewrite size_map size_to_list /max  /= => ib.
   rewrite !nth_cat !size_map !size_cat !size_map !size_iota /max /=. 
   case (i <256).
-  + move => ?;rewrite ifT 1:/#.
+  + move => ?;rewrite ifT 1:/# ifT 1:/#.
     rewrite (nth_map witness).
     + rewrite size_map size_chunk 1:/# (EclibExtra.size_flatten' 8);1:smt(mapP W8.size_w2bits). 
       rewrite size_map size_to_list /= /#.
@@ -771,21 +857,21 @@ have H3 :
     rewrite (nth_map witness _ ((W16.of_int \o asint))) /=.
     + rewrite size_to_list /= /#.
    rewrite /(\o) /= mapiE 1:/# /= initiE 1:/# /=.  
-  rewrite /(\o) /decompress10_circuit -decompress_alt_decompress /decompress_alt //=.
+  rewrite /(\o) /decompress11_circuit -decompress_alt_decompress /decompress_alt //=.
   rewrite get_of_list 1:/# /= qE /=.
-  have Hs := size_nth_chunk [] (flatten (map W8.w2bits (to_list ap{hr}))) i 10 _ _ => //.
+  have Hs := size_nth_chunk [] (flatten (map W8.w2bits (to_list ap{hr}))) i 11 _ _ => //.
   + rewrite (EclibExtra.size_flatten' 8);1:smt(mapP W8.size_w2bits). 
     by rewrite size_map size_to_list /#.
   rewrite to_uint_eq to_uint_truncateu16 /= /srl_32 /= of_uintK /=;congr;congr.
-  have ? : 2^10 = 1024 by auto.
-  rewrite to_uint_shr //= /zeroextu10_32 to_uintD_small /=;1: by rewrite of_uintK /=; smt(modz_small W10.to_uint_cmp). 
-  rewrite of_uintK /= modz_small;1:by smt( W10.to_uint_cmp). 
+  have ? : 2^11 = 2048 by auto.
+  rewrite to_uint_shr //= /zeroextu11_32 to_uintD_small /=;1: by rewrite of_uintK /=; smt(modz_small W11.to_uint_cmp). 
+  rewrite of_uintK /= modz_small;1:by smt( W11.to_uint_cmp). 
   rewrite /to_uint bits2wK 1:/# incoeffK qE /= /decode (nth_map [] _ bs2int) /=.
   + rewrite size_chunk 1:/# size_BytesToBits size_to_list /= /#.
-  by smt(BS2Int.bs2int_ge0 BS2Int.bs2int_le2Xs modz_small W10.to_uint_cmp). 
+  by smt(BS2Int.bs2int_ge0 BS2Int.bs2int_le2Xs modz_small W11.to_uint_cmp). 
 
   case (i <512).
-  + move => ??.
+  + move => ??;rewrite ifT 1:/#.
     rewrite (nth_map witness).
     + rewrite size_map size_chunk 1:/# (EclibExtra.size_flatten' 8);1:smt(mapP W8.size_w2bits). 
       rewrite size_map size_to_list /= /#.
@@ -795,20 +881,21 @@ have H3 :
     rewrite (nth_map witness _ ((W16.of_int \o asint))) /=.
     + rewrite size_to_list /= /#.
    rewrite /(\o) /= mapiE 1:/# /= initiE 1:/# /=.  
-  rewrite /(\o) /decompress10_circuit -decompress_alt_decompress /decompress_alt //=.
+  rewrite /(\o) /decompress11_circuit -decompress_alt_decompress /decompress_alt //=.
   rewrite get_of_list 1:/# /= qE /=.
-  have Hs := size_nth_chunk [] (flatten (map W8.w2bits (to_list ap{hr}))) i 10 _ _ => //.
+  have Hs := size_nth_chunk [] (flatten (map W8.w2bits (to_list ap{hr}))) i 11 _ _ => //.
   + rewrite (EclibExtra.size_flatten' 8);1:smt(mapP W8.size_w2bits). 
     by rewrite size_map size_to_list /#.
   rewrite to_uint_eq to_uint_truncateu16 /= /srl_32 /= of_uintK /=;congr;congr.
-  have ? : 2^10 = 1024 by auto.
-  rewrite to_uint_shr //= /zeroextu10_32 to_uintD_small /=;1: by rewrite of_uintK /=; smt(modz_small W10.to_uint_cmp). 
-  rewrite of_uintK /= modz_small;1:by smt( W10.to_uint_cmp). 
+  have ? : 2^11 = 2048 by auto.
+  rewrite to_uint_shr //= /zeroextu11_32 to_uintD_small /=;1: by rewrite of_uintK /=; smt(modz_small W11.to_uint_cmp). 
+  rewrite of_uintK /= modz_small;1:by smt( W11.to_uint_cmp). 
   rewrite /to_uint bits2wK 1:/# incoeffK qE /= /decode (nth_map [] _ bs2int) /=.
   + rewrite size_chunk 1:/# size_BytesToBits size_to_list /= /#.
-  by smt(BS2Int.bs2int_ge0 BS2Int.bs2int_le2Xs modz_small W10.to_uint_cmp). 
+  by smt(BS2Int.bs2int_ge0 BS2Int.bs2int_le2Xs modz_small W11.to_uint_cmp). 
 
-  + move => ??.
+  case (i <768).
+  + move => ???.
     rewrite (nth_map witness).
     + rewrite size_map size_chunk 1:/# (EclibExtra.size_flatten' 8);1:smt(mapP W8.size_w2bits). 
       rewrite size_map size_to_list /= /#.
@@ -818,24 +905,47 @@ have H3 :
     rewrite (nth_map witness _ ((W16.of_int \o asint))) /=.
     + rewrite size_to_list /= /#.
    rewrite /(\o) /= mapiE 1:/# /= initiE 1:/# /=.  
-  rewrite /(\o) /decompress10_circuit -decompress_alt_decompress /decompress_alt //=.
+  rewrite /(\o) /decompress11_circuit -decompress_alt_decompress /decompress_alt //=.
   rewrite get_of_list 1:/# /= qE /=.
-  have Hs := size_nth_chunk [] (flatten (map W8.w2bits (to_list ap{hr}))) i 10 _ _ => //.
+  have Hs := size_nth_chunk [] (flatten (map W8.w2bits (to_list ap{hr}))) i 11 _ _ => //.
   + rewrite (EclibExtra.size_flatten' 8);1:smt(mapP W8.size_w2bits). 
     by rewrite size_map size_to_list /#.
   rewrite to_uint_eq to_uint_truncateu16 /= /srl_32 /= of_uintK /=;congr;congr.
-  have ? : 2^10 = 1024 by auto.
-  rewrite to_uint_shr //= /zeroextu10_32 to_uintD_small /=;1: by rewrite of_uintK /=; smt(modz_small W10.to_uint_cmp). 
-  rewrite of_uintK /= modz_small;1:by smt( W10.to_uint_cmp). 
+  have ? : 2^11 = 2048 by auto.
+  rewrite to_uint_shr //= /zeroextu11_32 to_uintD_small /=;1: by rewrite of_uintK /=; smt(modz_small W11.to_uint_cmp). 
+  rewrite of_uintK /= modz_small;1:by smt( W11.to_uint_cmp). 
   rewrite /to_uint bits2wK 1:/# incoeffK qE /= /decode (nth_map [] _ bs2int) /=.
   + rewrite size_chunk 1:/# size_BytesToBits size_to_list /= /#.
-  by smt(BS2Int.bs2int_ge0 BS2Int.bs2int_le2Xs modz_small W10.to_uint_cmp). 
+  by smt(BS2Int.bs2int_ge0 BS2Int.bs2int_le2Xs modz_small W11.to_uint_cmp). 
+
+  + move => ???.
+    rewrite (nth_map witness).
+    + rewrite size_map size_chunk 1:/# (EclibExtra.size_flatten' 8);1:smt(mapP W8.size_w2bits). 
+      rewrite size_map size_to_list /= /#.
+    rewrite (nth_map []).
+    + rewrite  size_chunk 1:/# (EclibExtra.size_flatten' 8);1:smt(mapP W8.size_w2bits). 
+      rewrite size_map size_to_list /= /#.
+    rewrite (nth_map witness _ ((W16.of_int \o asint))) /=.
+    + rewrite size_to_list /= /#.
+   rewrite /(\o) /= mapiE 1:/# /= initiE 1:/# /=.  
+  rewrite /(\o) /decompress11_circuit -decompress_alt_decompress /decompress_alt //=.
+  rewrite get_of_list 1:/# /= qE /=.
+  have Hs := size_nth_chunk [] (flatten (map W8.w2bits (to_list ap{hr}))) i 11 _ _ => //.
+  + rewrite (EclibExtra.size_flatten' 8);1:smt(mapP W8.size_w2bits). 
+    by rewrite size_map size_to_list /#.
+  rewrite to_uint_eq to_uint_truncateu16 /= /srl_32 /= of_uintK /=;congr;congr.
+  have ? : 2^11 = 2048 by auto.
+  rewrite to_uint_shr //= /zeroextu11_32 to_uintD_small /=;1: by rewrite of_uintK /=; smt(modz_small W11.to_uint_cmp). 
+  rewrite of_uintK /= modz_small;1:by smt( W11.to_uint_cmp). 
+  rewrite /to_uint bits2wK 1:/# incoeffK qE /= /decode (nth_map [] _ bs2int) /=.
+  + rewrite size_chunk 1:/# size_BytesToBits size_to_list /= /#.
+  by smt(BS2Int.bs2int_ge0 BS2Int.bs2int_le2Xs modz_small W11.to_uint_cmp). 
 
 
 split; last first.
 + rewrite eq_vectorP => i @/kvec ib.
   rewrite /lift_polyvec /decompress_polyvec !setvE !offunvE 1..2:/# /= !offunvK /vclamp /kvec /= ib /=. 
-  case (2 = i) => Hi.
+  case (3 = i) => Hi.
   + rewrite tP => k kb. 
     rewrite -Hi !mapiE 1,2:/# !initiE 1,2:/# /= /= -get_to_list H2 H3.
   rewrite (nth_map witness);1: by smt(Array256.size_to_list size_cat).
@@ -844,50 +954,77 @@ split; last first.
     rewrite !setvE !offunvE 1:/# /=.
     rewrite initiE 1:/# /= mapiE 1:/# initiE 1:/# /=.
     rewrite get_of_list 1:/# /=.
-  pose c := (decompress 10 (nth 0 (decode 10 (to_list ap{hr})) (512 + k))).
+  pose c := (decompress 11 (nth 0 (decode 11 (to_list ap{hr})) (768 + k))).
   rewrite of_sintK /= /smod /= ifF;1:smt(@Zq).
   rewrite modz_small; smt(@Zq).  
+
+  case (2 = i) => Hi2.
+  + rewrite tP => k kb. 
+    rewrite -Hi2 !mapiE 1,2:/# !initiE 1,2:/# /= /= -get_to_list H2 H3.
+  rewrite (nth_map witness);1: by smt(Array256.size_to_list size_cat).
+  rewrite (nth_cat witness).
+  + rewrite !size_cat !size_to_list /= ifT 1:/# /decompress_polyvec.
+    rewrite !setvE !offunvE 1..3:/# /=  !offunvK /vclamp /= !ifT 1..6:/#.
+  rewrite (nth_cat witness).
+  + rewrite !size_cat !size_to_list /= ifF 1:/# /decompress_polyvec.
+    rewrite  mapiE 1:/# initiE 1:/# /= initiE 1:/# /=.
+    rewrite of_sintK /= /smod /= ifF;1:smt(@Zq).
+  rewrite /decode11_vec get_of_list 1:/#.
+  pose c := decompress 11 (nth 0 (decode 11 (to_list ap{hr})) (512 + k)).
+  rewrite modz_small; smt(@Zq).  
+
   case (1 = i) => Hi1.
   + rewrite tP => k kb. 
     rewrite -Hi1 !mapiE 1,2:/# !initiE 1,2:/# /= /= -get_to_list H2 H3.
   rewrite (nth_map witness);1: by smt(Array256.size_to_list size_cat).
   rewrite (nth_cat witness).
   + rewrite !size_cat !size_to_list /= ifT 1:/# /decompress_polyvec.
-    rewrite !setvE !offunvE 1,2:/# /= !offunvK /vclamp /= !ifT 1..3:/#.
+    rewrite !setvE !offunvE 1..3:/# /= !offunvK /vclamp /= !ifT 1..6:/#.
+  rewrite (nth_cat witness).
+  + rewrite !size_cat !size_to_list /= ifT 1:/# /decompress_polyvec.
   rewrite (nth_cat witness).
   + rewrite !size_to_list /= ifF 1:/# /decompress_polyvec.
-    rewrite initiE 1:/# /= mapiE 1:/# initiE 1:/# /=.
-    rewrite get_of_list 1:/# /=.
-  pose c := (decompress 10 (nth 0 (decode 10 (to_list ap{hr})) (256 + k))).
-  rewrite of_sintK /= /smod /= ifF;1:smt(@Zq).
+    rewrite  mapiE 1:/# initiE 1:/# /= initiE 1:/# /=.
+    rewrite of_sintK /= /smod /= ifF;1:smt(@Zq).
+  rewrite /decode11_vec get_of_list 1:/#.
+    pose c := (decompress 11 (nth 0 (decode 11 (to_list ap{hr})) (256 + k))).
   rewrite modz_small; smt(@Zq).  
-  have Hi2 :(0 = i) by smt().
+
+  have Hi3 :(0 = i) by smt().
   + rewrite tP => k kb. 
-    rewrite -Hi2 !mapiE 1:/# /= !initiE 1:/# /= /= -get_to_list H2 H3.
+    rewrite -Hi3 !mapiE 1:/# /= !initiE 1:/# /= /= -get_to_list H2 H3.
   rewrite (nth_map witness);1: by smt(Array256.size_to_list size_cat).
   rewrite (nth_cat witness).
   + rewrite !size_cat !size_to_list /= ifT 1:/# /decompress_polyvec.
-    rewrite !setvE !offunvE 1,2:/# /= !offunvK /vclamp /= !ifT 1..3:/#.
+    rewrite !setvE !offunvE 1..3:/# /= !offunvK /vclamp /= !ifT 1..6:/#.
+  rewrite (nth_cat witness).
+  + rewrite !size_cat !size_to_list /= ifT 1:/# /decompress_polyvec.
   rewrite (nth_cat witness).
   + rewrite !size_to_list /= ifT 1:/# /decompress_polyvec.
-    rewrite mapiE 1:/# initiE 1:/# /=. 
-  pose c :=(decompress 10 (decode10_vec ap{hr}).[k]).
-  rewrite of_sintK /= /smod /= ifF;1:smt(@Zq).
+    rewrite  mapiE 1:/# initiE 1:/# /= initiE 1:/# /=.
+    rewrite of_sintK /= /smod /= ifF;1:smt(@Zq).
+    pose c := (decompress 11 (nth 0 (decode 11 (to_list ap{hr})) (k))).
   rewrite modz_small; smt(@Zq).  
 
 
-rewrite /pos_bound768_cxq qE /= => k kb. 
+rewrite /pos_bound1024_cxq qE /= => k kb. 
 rewrite -get_to_list  H2 H3 /decompress_poly.
 rewrite (nth_map witness);1: by smt(size_cat Array256.size_to_list).
 rewrite (nth_cat witness) !size_cat !size_to_list /=. 
+rewrite (nth_cat witness) !size_cat !size_to_list /=. 
 rewrite (nth_cat witness)  !size_to_list /=. 
-rewrite /decompress_polyvec !setvE /= !offunvE 1..3:/# /= !offunvK /= /vclamp /kvec/=.
+rewrite /decompress_polyvec !setvE /= !offunvE 1..4:/# /= !offunvK /= /vclamp /kvec/=.
 case (k < 256).
 + move => *; rewrite ifT 1:/# .
   rewrite mapiE 1:/# initiE 1:/# /=.
   rewrite of_sintK /= /smod /= ifF;1:smt(@Zq).
   rewrite modz_small; smt(@Zq).  
 case (k < 512).
++ move => *.
+  rewrite mapiE 1:/# initiE 1:/# /=.
+  rewrite of_sintK /= /smod /= ifF;1:smt(@Zq).
+  rewrite modz_small; smt(@Zq).  
+case (k < 768).
 + move => *.
   rewrite mapiE 1:/# initiE 1:/# /=.
   rewrite of_sintK /= /smod /= ifF;1:smt(@Zq).
@@ -903,11 +1040,11 @@ qed.
 
 
 lemma polyvec_decompress_corr _aw :
-    phoare [Jkem768.M.__i_polyvec_decompress  :
+    phoare [Jkem1024.M.__i_polyvec_decompress  :
              ap = _aw
               ==>
-             pos_bound768_cxq res 0 768 1 /\
-             lift_polyvec res = decompress_polyvec 10 (decode10_vec _aw) ] = 1%r
+             pos_bound1024_cxq res 0 1024 1 /\
+             lift_polyvec res = decompress_polyvec 11 (decode11_vec _aw) ] = 1%r
   by conseq polyvec_decompress_ll (polyvec_decompress_corr_h _aw).
 
 
@@ -917,17 +1054,17 @@ op frombytes_circuit(c : W12.t) : W16.t =
   zeroextu16 c.
 
 
-lemma polyvec_frombytes_ll : islossless Jkem768.M.__i_polyvec_frombytes.
+lemma polyvec_frombytes_ll : islossless Jkem1024.M.__i_polyvec_frombytes.
 proc; inline *;wp. 
-  while (0 <= i <= 3) (3-i); last by  auto =>  /> /#.
+  while (0 <= i <= 4) (4-i); last by  auto =>  /> /#.
 move => *. cfold 3. unroll for ^while;auto => /> /#.
 qed.
 
 lemma decode_range_vec dfl (l : W8.t list) n :
   1 < n <= 12 =>
-    size l = 768*n %/ 8 =>
-  size (decode n l) = 768 /\
-  (forall k, 0<=k<768 => 0<= nth dfl (decode n l) k <2^n).
+    size l = 1024*n %/ 8 =>
+  size (decode n l) = 1024 /\
+  (forall k, 0<=k<1024 => 0<= nth dfl (decode n l) k <2^n).
 move => *.
 rewrite -andaE;split;1: by rewrite /decode size_map size_chunk 1:/# size_BytesToBits /#. 
 move => ? k kb.
@@ -937,23 +1074,23 @@ rewrite (nth_map witness);1: by rewrite size_chunk 1:/# size_BytesToBits /#.
 smt(BS2Int.bs2int_ge0 BS2Int.bs2int_le2Xs).
 qed.
 
-lemma polyvec_frombytes_corr_h (_aw : W8.t Array1152.t): 
-    hoare [Jkem768.M.__i_polyvec_frombytes  :
+lemma polyvec_frombytes_corr_h (_aw : W8.t Array1536.t): 
+    hoare [Jkem1024.M.__i_polyvec_frombytes  :
              ap = _aw
               ==>
-             lift_array768 res = map incoeff (decode12_vec _aw)  /\
-             pos_bound768_cxq res 0 768  2].
+             lift_array1024 res = map incoeff (decode12_vec _aw)  /\
+             pos_bound1024_cxq res 0 1024  2].
 proc; inline *.
-proc change 1: (init_768_16 (fun _ => W16.zero));1: by admit.
+proc change 1: (init_1024_16 (fun _ => W16.zero));1: by admit.
 proc change ^while.1: (init_256_16 (fun (i_0 : int) => r.[256 * i + i_0])); 1: by auto.
 proc change ^while.2: (init_384_8 (fun (i_0 : int) => ap.[384 * i + i_0])  ); 1: by auto.
 proc change ^while.^while.7: (sll_16 t (W16.of_int 8)); 1: by auto.
 proc change ^while.^while.10: (sll_16 d1 (W16.of_int 4)); 1: by auto.
 proc change ^while.^while.12: (srl_16 t (W16.of_int 4)); 1: by auto.
-proc change ^while.7: (init_768_16 (fun (i_0 : int) => if 256 * i <= i_0 < 256 * i + 256 then aux.[i_0 - 256 * i] else r.[i_0])); 1: by auto.
+proc change ^while.7: (init_1024_16 (fun (i_0 : int) => if 256 * i <= i_0 < 256 * i + 256 then aux.[i_0 - 256 * i] else r.[i_0])); 1: by auto.
 unroll for ^while.
 cfold 4.
-do 3!(unroll for ^while).
+do 4!(unroll for ^while).
 cfold ^i0<-.
 wp -3.
 bdep 12 16 [_aw] [ap] [r] frombytes_circuit pcond_true12. 
@@ -966,15 +1103,14 @@ bdep 12 16 [_aw] [ap] [r] frombytes_circuit pcond_true12.
 (* We start with some boilerplate *)
 move => &hr [#]/= <- rr; rewrite /= !flatten1.
 move => H1; have H2 := post_lane_commute_out_aligned (to_list ap{hr}) (to_list rr) W8.w2bits W8.bits2w W12.w2bits W12.bits2w W16.w2bits W16.bits2w  frombytes_circuit 8 12 16 _ _ _ _ _ _ _ _ _ _ _ _ H1;1..12:
-smt(Array1152.size_to_list Array768.size_to_list W16.bits2wK BVA_Top_Bindings_W12_t.oflistP).
+smt(Array1536.size_to_list Array1024.size_to_list W16.bits2wK BVA_Top_Bindings_W12_t.oflistP).
 
-print decode_range.
-  have /=? := decode_range_vec 0 (to_list ap{hr}) 12 _ _;1,2:smt(Array1152.size_to_list).
+  have /=? := decode_range_vec 0 (to_list ap{hr}) 12 _ _;1,2:smt(Array1536.size_to_list).
 
 have H3 : 
   map frombytes_circuit (map W12.bits2w (chunk 12 (flatten (map W8.w2bits (to_list ap{hr}))))) =
    to_list (map W16.of_int  (decode12_vec ap{hr})).
-+ rewrite /decode12_vec Array768.map_of_list Array768.of_listK;1: smt(size_map). 
++ rewrite /decode12_vec Array1024.map_of_list Array1024.of_listK;1: smt(size_map). 
   rewrite /decode -map_comp -(map_comp _ BS2Int.bs2int) /=.
   apply eq_in_map => x xb.
   rewrite /(\o) /frombytes_circuit /zeroextu16.
@@ -989,8 +1125,8 @@ split.
   rewrite get_to_list mapiE 1:/# get_of_list 1:/# of_sintK /=.
   by rewrite /smod /= ifF 1:/# modz_small 1:/#.
 
-  rewrite /pos_bound768_cxq qE /= => k kb. 
-  have /=? := decode_range_vec witness (to_list ap{hr}) 12 _ _;1..2:smt(Array1152.size_to_list).
+  rewrite /pos_bound1024_cxq qE /= => k kb. 
+  have /=? := decode_range_vec witness (to_list ap{hr}) 12 _ _;1..2:smt(Array1536.size_to_list).
   rewrite -get_to_list  H2 H3 /decode12_vec.
   rewrite get_to_list /= get_of_list 1:/#.
   rewrite (nth_map witness) 1:/#.  
@@ -1003,24 +1139,25 @@ qed.
 (********** END BDEP PROOF OF FROMBYTES **************)
 
 lemma polyvec_frombytes_corr _aw :
-    phoare [ Jkem768.M.__i_polyvec_frombytes :
+    phoare [ Jkem1024.M.__i_polyvec_frombytes :
              ap = _aw
               ==>
-             lift_array768 res = map incoeff (decode12_vec _aw)  /\
-             pos_bound768_cxq res 0 768  2 ] = 1%r
+             lift_array1024 res = map incoeff (decode12_vec _aw)  /\
+             pos_bound1024_cxq res 0 1024  2 ] = 1%r
    by conseq polyvec_frombytes_ll (polyvec_frombytes_corr_h _aw).
 
 (******************************************************)
 
 
 lemma polyvec_tobytes_corr_h  _aw :
-    hoare [Jkem768.M.__i_polyvec_tobytes  :
-             pos_bound768_cxq a 0 768 2 /\
+    hoare [Jkem1024.M.__i_polyvec_tobytes  :
+             pos_bound1024_cxq a 0 1024 2 /\
              a = _aw 
               ==>
-             res = encode12_vec (map asint (lift_array768 _aw))
+             res = encode12_vec (map asint (lift_array1024 _aw))
               ].
 proc;unroll for 3.
+wp;call (poly_tobytes_corr_h (subarray256 _aw 3)).
 wp;call (poly_tobytes_corr_h (subarray256 _aw 2)).
 wp;call (poly_tobytes_corr_h (subarray256 _aw 1)).
 wp;call (poly_tobytes_corr_h (subarray256 _aw 0)).
@@ -1029,9 +1166,41 @@ move => ?;rewrite /subarray256 tP => Hin1 rr1 Hres1.
 split;1: by smt(Array256.initiE).
 move => ?;rewrite /subarray256 tP => Hin2 rr2 Hres2.
 split;1: by smt(Array256.initiE).
-move => ?;rewrite /subarray256 /encode12_vec tP => Hin3 rr3 Hres3.
+move => ?;rewrite /subarray256 tP => Hin3 rr3 Hres3.
+split;1: by smt(Array256.initiE).
+move => ?;rewrite /subarray256 /encode12_vec tP => Hin4 rr4 Hres4.
 rewrite tP => k kb; rewrite initiE 1:/# /= get_of_list 1:/# /=. 
-case (768 <= k < 1152).
+case (1152 <= k < 1536).
++ move => ?.
+  rewrite Hres4 /encode12 /encode get_of_list 1:/# /BitsToBytes.
+  rewrite (nth_map []).
+  + rewrite size_chunk 1:/# (EclibExtra.size_flatten' 12);1: smt(mapP size_int2bs).
+  by rewrite size_map size_to_list /#.
+  rewrite (nth_map []).
+  + rewrite size_chunk 1:/# (EclibExtra.size_flatten' 12);1: smt(mapP size_int2bs).
+  by rewrite size_map size_to_list /#.
+  congr; rewrite !JWordList.nth_chunk 1,2,4,5:/#. 
+  + rewrite (EclibExtra.size_flatten' 12);1: smt(mapP size_int2bs).
+    by rewrite size_map size_to_list /#.
+  + rewrite (EclibExtra.size_flatten' 12);1: smt(mapP size_int2bs).
+    by rewrite size_map size_to_list /#.
+  apply (eq_from_nth witness).
+  + rewrite !size_take 1,2:/# !size_drop 1,2:/# !(EclibExtra.size_flatten' 12);1,2: smt(mapP size_int2bs).
+    rewrite !size_map !size_iota /= /#.  
+  move => i.
+  + rewrite !size_take 1:/# !size_drop 1:/# !(EclibExtra.size_flatten' 12);1: smt(mapP size_int2bs).
+    rewrite !size_map !size_iota /= /max/= => ?. 
+  rewrite !nth_take 1..4:/# !nth_drop 1..4:/#. 
+  rewrite (nth_flatten witness 12) => /=.
+  + rewrite allP => * /=;smt(mapP size_int2bs). 
+  rewrite (nth_flatten witness 12) => /=.
+  + rewrite allP => * /=;smt(mapP size_int2bs). 
+  rewrite (nth_map witness _ _ ((8 * (k - 1152) + i) %/ 12));1:smt(Array256.size_to_list).
+  rewrite (nth_map witness _ _ ((8 * k + i) %/ 12));1:smt(Array1024.size_to_list).
+  rewrite !get_to_list !mapiE 1..4:/# /= initiE /#.
+
+move => ?;rewrite initiE 1:/# /=.
+case (768 <= k < 1152 ).
 + move => ?.
   rewrite Hres3 /encode12 /encode get_of_list 1:/# /BitsToBytes.
   rewrite (nth_map []).
@@ -1057,7 +1226,7 @@ case (768 <= k < 1152).
   rewrite (nth_flatten witness 12) => /=.
   + rewrite allP => * /=;smt(mapP size_int2bs). 
   rewrite (nth_map witness _ _ ((8 * (k - 768) + i) %/ 12));1:smt(Array256.size_to_list).
-  rewrite (nth_map witness _ _ ((8 * k + i) %/ 12));1:smt(Array768.size_to_list).
+  rewrite (nth_map witness _ _ ((8 * k + i) %/ 12));1:smt(Array1024.size_to_list).
   rewrite !get_to_list !mapiE 1..4:/# /= initiE /#.
 
 move => ?;rewrite initiE 1:/# /=.
@@ -1087,7 +1256,7 @@ case (384 <= k < 768 ).
   rewrite (nth_flatten witness 12) => /=.
   + rewrite allP => * /=;smt(mapP size_int2bs). 
   rewrite (nth_map witness _ _ ((8 * (k - 384) + i) %/ 12));1:smt(Array256.size_to_list).
-  rewrite (nth_map witness _ _ ((8 * k + i) %/ 12));1:smt(Array768.size_to_list).
+  rewrite (nth_map witness _ _ ((8 * k + i) %/ 12));1:smt(Array1024.size_to_list).
   rewrite !get_to_list !mapiE 1..4:/# /= initiE /#.
 
 move => ?;rewrite initiE 1:/# /=; rewrite ifT 1:/# /=.
@@ -1115,51 +1284,56 @@ move => ?;rewrite initiE 1:/# /=; rewrite ifT 1:/# /=.
   rewrite (nth_flatten witness 12) => /=.
   + rewrite allP => * /=;smt(mapP size_int2bs). 
   rewrite (nth_map witness _ _ ((8 * k  + i) %/ 12));1:smt(Array256.size_to_list).
-  rewrite (nth_map witness [] _  ((8 * k  + i) %/ 12)); 1:smt(Array768.size_to_list).
+  rewrite (nth_map witness [] _  ((8 * k  + i) %/ 12)); 1:smt(Array1024.size_to_list).
   rewrite !get_to_list !mapiE 1..4:/# /= initiE /#.
   qed.
 
 
-lemma polyvec_tobytes_ll  : islossless Jkem768.M.__i_polyvec_tobytes.
+lemma polyvec_tobytes_ll  : islossless Jkem1024.M.__i_polyvec_tobytes.
 proc. unroll for 3.
-do 3!(wp;call poly_tobytes_ll); auto.
+do 4!(wp;call poly_tobytes_ll); auto.
 qed.
 
 lemma polyvec_tobytes_corr  _aw : 
-    phoare [Jkem768.M.__i_polyvec_tobytes  :
-             pos_bound768_cxq a 0 768 2 /\
+    phoare [Jkem1024.M.__i_polyvec_tobytes  :
+             pos_bound1024_cxq a 0 1024 2 /\
              a = _aw 
               ==>
-             res = encode12_vec (map asint (lift_array768 _aw))
+             res = encode12_vec (map asint (lift_array1024 _aw))
               ] = 1%r
    by conseq polyvec_tobytes_ll (polyvec_tobytes_corr_h _aw).
 
 (******************************************************)
 
 lemma polyvec_ntt_correct_h _r:
-   hoare[Jkem768.M.__polyvec_ntt :
-        _r = r /\ signed_bound768_cxq r 0 768 2
+   hoare[Jkem1024.M.__polyvec_ntt :
+        _r = r /\ signed_bound1024_cxq r 0 1024 2
           ==> 
         nttv (lift_polyvec _r) = lift_polyvec res /\
-            pos_bound768_cxq res 0 768 2 ].
+            pos_bound1024_cxq res 0 1024 2 ].
 proof.
 proc.
 unroll for 2.
+wp;ecall (ntt_correct_h (lift_array256 (Array256.init (fun i => r.[(3 * 256) + i])))).
 wp;ecall (ntt_correct_h (lift_array256 (Array256.init (fun i => r.[(2 * 256) + i])))).
 wp;ecall (ntt_correct_h (lift_array256 (Array256.init (fun i => r.[256 + i])))).
 wp;ecall (ntt_correct_h (lift_array256 (Array256.init (fun i => r.[i])))).
-skip; move => &hr; rewrite /signed_bound_cxq /signed_bound768_cxq => [# _r_def signed_bound_r].
+skip; move => &hr; rewrite /signed_bound_cxq /signed_bound1024_cxq => [# _r_def signed_bound_r].
 
 split; 1: by auto => />;move => k kb kbl; rewrite initiE /#.
 
 move =>  [#] r_eq_res1 ? res1 [#] res1v signed_bound_res1 res1_eq_res2.
-split;1:by auto => />;move => k kb kbl; rewrite initiE 1:/# /=;smt(Array768.tP Array768.initiE).
+split;1:by auto => />;move => k kb kbl; rewrite initiE 1:/# /=;smt(Array1024.tP Array1024.initiE).
 
-move => signed_bound_r2 res2 [#] r_eq_res2 ? signed_bound_res2 />.
+move => signed_bound_r2 res2 [#] r_eq_res2  signed_bound_res2 /=.
 
-split; 1: by move => k k_bl kbh; rewrite !initiE 1:/# /= !initiE 1:/# /= !Array768.initiE 1:/# /= (fun_if W16.to_sint) /#.
+split; 1: by move => k k_bl; rewrite !initiE 1:/# /= !initiE 1:/# /= !Array1024.initiE 1:/# /= (fun_if W16.to_sint) /#.
 
-move => signed_bound_r3 res3 r_eq_res3 signed_bound_res3 />.
+move => signed_bound_r3 res3 [#] r_eq_res3 signed_bound_res3 /=.
+rewrite !andabP.
+split; 1: by move => k k_bl; rewrite !initiE 1:/# /= !initiE 1:/# /= !initiE 1:/# /= !initiE 1:/# /= (fun_if W16.to_sint) /#.
+
+move => res4 [#] r_eq_res4 signed_bound_res4 /=.
 
 split.
   rewrite /nttv /lift_polyvec !mapvE /= offunvK /vclamp /= eq_vectorP => k k_b.
@@ -1170,59 +1344,75 @@ split.
     rewrite k_v /= i_b /=.
     have ->: !(256 <= i && i < 512). move : i_b => /#.
     have ->: !(512 <= i && i < 768). move : i_b => /#.
+    have ->: !(768 <= i && i < 1024). move : i_b => /#.
     rewrite (lift_array256_incoeff res1) 1:/# /= -res1v r_eq_res1 /= _r_def.
     congr. congr.
     apply Array256.tP => j j_b.
     by rewrite -lift_array256_incoeff 1:j_b initiE 1:j_b /= /lift_array256 /= mapiE // initiE 1:j_b //.
+
   move : k_v => ?.
   case (k = 1) => k_v.
     rewrite k_v /=.
     have ->: (256 <= 256 + i && 256 + i < 512). move : i_b => /#.
     have ->: !(512 <= 256 + i && 256 + i < 768). move : i_b => /#.
+   have ->: !(768 <= 256+i && 256+i < 1024). move : i_b => /#.
     rewrite (lift_array256_incoeff res2) 1:/# -r_eq_res2 /= _r_def /lift_array256  //.
     congr. congr.
     apply Array256.tP => j j_b.
     rewrite -lift_array256_incoeff 1:j_b mapiE //=.
-    do (rewrite initiE 1:/# /=).
+    rewrite initiE 1:/# /= initiE 1:/# /= /res1_eq_res2 initiE 1:/# /=.
     have ->: !(0 <= 256 + j && 256 + j < 256). move : j_b => /#.
     by trivial.
   move : k_v => ?.
   case (k = 2) => k_v.
     rewrite k_v /=.
     have ->: (512 <= 512 + i && 512 + i < 768). move : i_b => /#.
+    have ->: !(768 <= 512 + i && 512 + i < 1024). move : i_b => /#.
     rewrite (lift_array256_incoeff res3) 1:/# -r_eq_res3 /= _r_def.
     congr. congr.
     apply Array256.tP => j j_b.
     rewrite -lift_array256_incoeff 1:j_b mapiE //=.
     do (rewrite initiE 1:/# /=).
     by smt().
+
+  move : k_v => ?.
+  case (k = 3) => k_v.
+    rewrite k_v /=.
+    have ->: (768 <= 768 + i && 768 + i < 1024). move : i_b => /#.
+    rewrite (lift_array256_incoeff res4) 1:/# -r_eq_res4 /= _r_def.
+    congr. congr.
+    apply Array256.tP => j j_b.
+    rewrite -lift_array256_incoeff 1:j_b mapiE //=.
+    do (rewrite initiE 1:/# /=).
+    by smt().
+
   by smt().
 
-  rewrite /pos_bound768_cxq => k k_b.
+  rewrite /pos_bound1024_cxq => k k_b.
   do (rewrite initiE 1:k_b /= || rewrite (fun_if W16.to_sint)).
-  move : (signed_bound_res3 (k - 512)) (signed_bound_res3 (k - 256)) (signed_bound_res1 k).
+  move : (signed_bound_res4 (k - 768)) (signed_bound_res3 (k - 512)) (signed_bound_res3 (k - 256)) (signed_bound_res1 k).
   by smt().
 qed.
 
-lemma polyvec_ntt_ll  : islossless Jkem768.M.__polyvec_ntt by  proc;unroll for 2;do 3! (wp;call(ntt_ll)).
+lemma polyvec_ntt_ll  : islossless Jkem1024.M.__polyvec_ntt by  proc;unroll for 2;do 4! (wp;call(ntt_ll)).
 
 lemma polyvec_ntt_corr _r:
-   phoare[Jkem768.M.__polyvec_ntt :
-        _r = r /\ signed_bound768_cxq r 0 768 2
+   phoare[Jkem1024.M.__polyvec_ntt :
+        _r = r /\ signed_bound1024_cxq r 0 1024 2
           ==> 
        nttv (lift_polyvec _r) = lift_polyvec res /\
-            pos_bound768_cxq res 0 768 2 ]  = 1%r 
+            pos_bound1024_cxq res 0 1024 2 ]  = 1%r 
 by conseq polyvec_ntt_ll (polyvec_ntt_correct_h _r).
 
 (******************************************************)
 
 lemma polyvec_invntt_correct_h _r:
-   hoare[Jkem768.M.__polyvec_invntt :
+   hoare[Jkem1024.M.__polyvec_invntt :
         _r = r /\
-        signed_bound768_cxq r 0 768 4
+        signed_bound1024_cxq r 0 1024 4
           ==> 
             scale_polyvec (invnttv (lift_polyvec _r)) (incoeff Fq.SignedReductions.R) = lift_polyvec res /\
-            forall (k : int), 0 <= k && k < 768 => b16 res.[k] (q) ].
+            forall (k : int), 0 <= k && k < 1024 => b16 res.[k] (q) ].
 proof.
 proc.
 unroll for 2.
@@ -1230,16 +1420,16 @@ wp;ecall (invntt_correct_h (lift_array256 (Array256.init (fun i => r.[(2 * 256) 
 wp;ecall (invntt_correct_h (lift_array256 (Array256.init (fun i => r.[256 + i])))).
 wp;ecall (invntt_correct_h (lift_array256 (Array256.init (fun i => r.[i])))).
 
-wp; skip; move => &hr; rewrite /signed_bound_cxq /signed_bound768_cxq => [ #_r_def signed_bound_r] *.
+wp; skip; move => &hr; rewrite /signed_bound_cxq /signed_bound1024_cxq => [ #_r_def signed_bound_r] *.
 
 split; 1: by auto => />;move => k kb kbl; rewrite initiE /#.
 
 move =>  [#] r_eq_res1 ? res1 [#] res1v signed_bound_res1 res1_eq_res2.
-split;1:by auto => />;move => k kb kbl; rewrite initiE 1:/# /=;smt(Array768.tP Array768.initiE).
+split;1:by auto => />;move => k kb kbl; rewrite initiE 1:/# /=;smt(Array1024.tP Array1024.initiE).
 
 move => signed_bound_r2 res2 [#] r_eq_res2 ? signed_bound_res2 />.
 
-split; 1: by move => k k_bl kbh; rewrite !initiE 1:/# /= !initiE 1:/# /= !Array768.initiE 1:/# /= (fun_if W16.to_sint) /#.
+split; 1: by move => k k_bl kbh; rewrite !initiE 1:/# /= !initiE 1:/# /= !Array1024.initiE 1:/# /= (fun_if W16.to_sint) /#.
 
 move => signed_bound_r3 res3 r_eq_res3 signed_bound_res3 />.
 
@@ -1253,14 +1443,14 @@ split.
   + move => k_v.
     rewrite k_v /= i_b /=.
     have ->: !(256 <= i && i < 512). move : i_b => /#.
-    have ->: !(512 <= i && i < 768). move : i_b => /#.
+    have ->: !(512 <= i && i < 1024). move : i_b => /#.
     by rewrite /= (lift_array256_incoeff res1) 1:/# -res1v -r_eq_res1 /= _r_def 
                    /lift_array256  //= mapiE //=.
   move => ?.
   case (k = 1) => k_v.
     rewrite k_v /=.
     have ->: (256 <= 256 + i && 256 + i < 512). move : i_b => /#.
-    have ->: !(512 <= 256 + i && 256 + i < 768). move : i_b => /#.
+    have ->: !(512 <= 256 + i && 256 + i < 1024). move : i_b => /#.
     rewrite (lift_array256_incoeff res2) 1:/# -r_eq_res2 /= _r_def
          /lift_array256  //= mapiE //=.
     congr;congr;congr.
@@ -1272,7 +1462,7 @@ split.
   move : k_v => ?.
   case (k = 2) => k_v.
     rewrite k_v /=.
-    have ->: (512 <= 512 + i && 512 + i < 768). move : i_b => /#.
+    have ->: (512 <= 512 + i && 512 + i < 1024). move : i_b => /#.
     rewrite (lift_array256_incoeff res3) 1:/# -r_eq_res3 /= _r_def
          /lift_array256  //= mapiE //=.
     congr;congr;congr.
@@ -1289,14 +1479,14 @@ split.
 qed.
 
 lemma polyvec_invntt_ll  :
-      islossless Jkem768.M.__polyvec_invntt by  proc;unroll for 2;do 3! (wp;call(invntt_ll)).
+      islossless Jkem1024.M.__polyvec_invntt by  proc;unroll for 2;do 3! (wp;call(invntt_ll)).
 
 lemma polyvec_invntt_corr _r:
-   phoare[Jkem768.M.__polyvec_invntt :
-    _r = r /\ signed_bound768_cxq r 0 768 4
+   phoare[Jkem1024.M.__polyvec_invntt :
+    _r = r /\ signed_bound1024_cxq r 0 1024 4
       ==> 
      scale_polyvec (invnttv (lift_polyvec _r)) (incoeff Fq.SignedReductions.R) = lift_polyvec res /\
-            forall (k : int), 0 <= k && k < 768 => b16 res.[k] (q) ]  = 1%r   
+            forall (k : int), 0 <= k && k < 1024 => b16 res.[k] (q) ]  = 1%r   
    by conseq polyvec_invntt_ll (polyvec_invntt_correct_h _r).
 
 (******************************************************)
@@ -1307,15 +1497,15 @@ lemma polyvec_pointwise_acc_corr_h _a0 _a1 _a2 _b0 _b1 _b2 _p0 _p1 _p2 (_r : coe
   _p2 = scale (basemul _a2 _b2) (incoeff 169) =>
   (forall k, 0 <=  k < 256 =>
      _r.[k] = _p0.[k] + _p1.[k] + _p2.[k])  =>
-  hoare [Jkem768.M.__polyvec_pointwise_acc : 
-    _a0 = subarray256 (lift_array768 a) 0 /\
-    _a1 = subarray256 (lift_array768 a) 1 /\
-    _a2 = subarray256 (lift_array768 a) 2 /\
-    _b0 = subarray256 (lift_array768 b) 0 /\
-    _b1 = subarray256 (lift_array768 b) 1 /\
-    _b2 = subarray256 (lift_array768 b)  2 /\
-    signed_bound768_cxq a 0 768 2 /\ 
-    signed_bound768_cxq b  0 768 2 
+  hoare [Jkem1024.M.__polyvec_pointwise_acc : 
+    _a0 = subarray256 (lift_array1024 a) 0 /\
+    _a1 = subarray256 (lift_array1024 a) 1 /\
+    _a2 = subarray256 (lift_array1024 a) 2 /\
+    _b0 = subarray256 (lift_array1024 b) 0 /\
+    _b1 = subarray256 (lift_array1024 b) 1 /\
+    _b2 = subarray256 (lift_array1024 b)  2 /\
+    signed_bound1024_cxq a 0 1024 2 /\ 
+    signed_bound1024_cxq b  0 1024 2 
      ==> 
     lift_array256 res =  _r /\
     forall (k : int), 0 <= k && k < 256 => 
@@ -1331,7 +1521,7 @@ have H:= (poly_add_corr_impl_h 3 3 _ _) => //; ecall (H _p0 _p1); clear H.
 call (poly_basemul_corr _a1 _b1).
 call (poly_basemul_corr _a0 _b0).
 
-wp; skip; subst => &hr; rewrite /subarray256 /lift_array768 /lift_array256 /signed_bound768_cxq /signed_bound_cxq /=  => [#].
+wp; skip; subst => &hr; rewrite /subarray256 /lift_array1024 /lift_array256 /signed_bound1024_cxq /signed_bound_cxq /=  => [#].
 
 move => _a0_def _a1_def _a2_def _b0_def _b1_def _b2_def  signed_bound_a signed_bound_b.
 
@@ -1339,7 +1529,7 @@ split.
 + rewrite _a0_def _b0_def mapE.
   split.
   + apply Array256.ext_eq => k kb.
-    by rewrite !initiE //= Array768.initiE /= 1:/# mapiE //= initiE //.
+    by rewrite !initiE //= Array1024.initiE /= 1:/# mapiE //= initiE //.
   split.
   +  apply Array256.ext_eq => k kb.
      by rewrite !initiE //= mapiE // 1: /# /= mapiE //= initiE //.
@@ -1350,7 +1540,7 @@ split.
 + rewrite _a1_def _b1_def mapE.
   split.
   + apply Array256.ext_eq => k kb.
-    by rewrite !initiE //= Array768.initiE /= 1:/# mapiE //= initiE //.
+    by rewrite !initiE //= Array1024.initiE /= 1:/# mapiE //= initiE //.
   split.
   +  apply Array256.ext_eq => k kb.
      by rewrite !initiE //= mapiE // 1: /# /= mapiE //= initiE //.
@@ -1366,7 +1556,7 @@ split.
 + rewrite _a2_def _b2_def /lift_polyvec /lift_array256 mapE.
   split.
   + apply Array256.ext_eq => k kb.
-    by rewrite !initiE //= Array768.initiE /= 1:/# mapiE //= initiE //.
+    by rewrite !initiE //= Array1024.initiE /= 1:/# mapiE //= initiE //.
   split.
   +  apply Array256.ext_eq => k kb.
      by rewrite !initiE //= mapiE // 1: /# /= mapiE //= initiE //.
@@ -1385,7 +1575,7 @@ by smt().
 qed.
 
 lemma polyvec_pointwise_acc_ll  :
-      islossless Jkem768.M.__polyvec_pointwise_acc
+      islossless Jkem1024.M.__polyvec_pointwise_acc
 by  proc;call poly_reduce_ll; unroll for 5;wp;do 2! (call poly_add_ll;call poly_basemul_ll); call poly_basemul_ll;auto.
 
 lemma polyvec_pointwise_acc_corr _a0 _a1 _a2 _b0 _b1 _b2 _p0 _p1 _p2 (_r : coeff Array256.t) :
@@ -1394,15 +1584,15 @@ lemma polyvec_pointwise_acc_corr _a0 _a1 _a2 _b0 _b1 _b2 _p0 _p1 _p2 (_r : coeff
   _p2 = scale (basemul _a2 _b2) (incoeff 169) =>
   (forall k, 0 <=  k < 256 =>
      _r.[k] = _p0.[k] + _p1.[k] + _p2.[k])  =>
-  phoare [Jkem768.M.__polyvec_pointwise_acc : 
-    _a0 = subarray256 (lift_array768 a) 0 /\
-    _a1 = subarray256 (lift_array768 a) 1 /\
-    _a2 = subarray256 (lift_array768 a) 2 /\
-    _b0 = subarray256 (lift_array768 b) 0 /\
-    _b1 = subarray256 (lift_array768 b) 1 /\
-    _b2 = subarray256 (lift_array768 b)  2 /\
-    signed_bound768_cxq a 0 768 2 /\ 
-    signed_bound768_cxq b  0 768 2 
+  phoare [Jkem1024.M.__polyvec_pointwise_acc : 
+    _a0 = subarray256 (lift_array1024 a) 0 /\
+    _a1 = subarray256 (lift_array1024 a) 1 /\
+    _a2 = subarray256 (lift_array1024 a) 2 /\
+    _b0 = subarray256 (lift_array1024 b) 0 /\
+    _b1 = subarray256 (lift_array1024 b) 1 /\
+    _b2 = subarray256 (lift_array1024 b)  2 /\
+    signed_bound1024_cxq a 0 1024 2 /\ 
+    signed_bound1024_cxq b  0 1024 2 
      ==> 
     lift_array256 res =  _r /\
     forall (k : int), 0 <= k && k < 256 => 
@@ -1414,11 +1604,11 @@ move => *;conseq polyvec_pointwise_acc_ll (polyvec_pointwise_acc_corr_h _a0 _a1 
 (******************************************************)
 
 lemma polyvec_pointwise_acc_corr_alg_h va vb :
-  hoare [Jkem768.M.__polyvec_pointwise_acc :
+  hoare [Jkem1024.M.__polyvec_pointwise_acc :
     nttv va = lift_polyvec a /\
     nttv vb = lift_polyvec b /\
-    signed_bound768_cxq a 0 768 2 /\
-    signed_bound768_cxq b 0 768 2
+    signed_bound1024_cxq a 0 1024 2 /\
+    signed_bound1024_cxq b 0 1024 2
     ==> 
     signed_bound_cxq res 0 256 2 /\
     lift_array256  res = scale (ntt (dotp va vb)) (incoeff 169)  ].
@@ -1434,7 +1624,7 @@ proof.
 by move => k; rewrite /(&+) map2E map2E /= initE /= initE //= /#.
 move => H; conseq (H).
 move => &hr.
-rewrite /nttv /lift_polyvec /lift_array256 /= /subarray256 /= /lift_array768 => />  H0 H1 H2 H3.
+rewrite /nttv /lift_polyvec /lift_array256 /= /subarray256 /= /lift_array1024 => />  H0 H1 H2 H3.
 move : H0 H1; rewrite !eq_vectorP => /> H0 H1. 
 do split.
 + move : (H0 0 _) => //=.
@@ -1477,21 +1667,21 @@ by ring.
 qed.
 
 lemma polyvec_pointwise_acc_corr_alg va vb :
-  phoare [Jkem768.M.__polyvec_pointwise_acc :
+  phoare [Jkem1024.M.__polyvec_pointwise_acc :
     nttv va = lift_polyvec a /\
     nttv vb = lift_polyvec b /\
-    signed_bound768_cxq a 0 768 2 /\
-    signed_bound768_cxq b 0 768 2
+    signed_bound1024_cxq a 0 1024 2 /\
+    signed_bound1024_cxq b 0 1024 2
     ==> 
     signed_bound_cxq res 0 256 2 /\
     lift_array256  res = scale (ntt (dotp va vb)) (incoeff 169)  ] = 1%r by
 move => *;conseq polyvec_pointwise_acc_ll (polyvec_pointwise_acc_corr_alg_h va vb) => //.
 
 module Aux = {
-   proc inner_product(ai skpv : W16.t Array768.t) : W16.t Array256.t = {
+   proc inner_product(ai skpv : W16.t Array1024.t) : W16.t Array256.t = {
         var polyi,r';
-        polyi <@ Jkem768.M.__polyvec_pointwise_acc(ai,skpv);
-        r' <@ Jkem768.M._poly_frommont(polyi);
+        polyi <@ Jkem1024.M.__polyvec_pointwise_acc(ai,skpv);
+        r' <@ Jkem1024.M._poly_frommont(polyi);
         return r';
    }
 }.
@@ -1502,8 +1692,8 @@ lemma innerprod_corr_h va vb:
   hoare [ Aux.inner_product :
     nttv va = lift_polyvec ai /\
     nttv vb = lift_polyvec skpv /\
-    signed_bound768_cxq ai 0 768 2 /\
-    signed_bound768_cxq skpv 0 768 2
+    signed_bound1024_cxq ai 0 1024 2 /\
+    signed_bound1024_cxq skpv 0 1024 2
     ==> 
     signed_bound_cxq res 0 256 2 /\
     lift_array256  res = ntt (dotp va vb)  ].
@@ -1516,7 +1706,7 @@ seq 1 : (#pre /\
 by call (polyvec_pointwise_acc_corr_alg_h va vb); auto => />.
 
 ecall(poly_frommont_corr_h (map W16.to_sint polyi)).
-skip => &hr; rewrite /lift_polyvec /signed_bound768_cxq  /lift_polyvec /lift_array256 /signed_bound_cxq /scale /= !tP /=.
+skip => &hr; rewrite /lift_polyvec /signed_bound1024_cxq  /lift_polyvec /lift_array256 /signed_bound_cxq /scale /= !tP /=.
 move => /> VA VB AB BB H H0. 
 
 split; 1: by move => k kbl kbh; move : (H k _) => //; rewrite !mapiE //=.
@@ -1551,8 +1741,8 @@ lemma innerprod_corr va vb:
   phoare [ Aux.inner_product :
     nttv va = lift_polyvec ai /\
     nttv vb = lift_polyvec skpv /\
-    signed_bound768_cxq ai 0 768 2 /\
-    signed_bound768_cxq skpv 0 768 2
+    signed_bound1024_cxq ai 0 1024 2 /\
+    signed_bound1024_cxq skpv 0 1024 2
     ==> 
     signed_bound_cxq res 0 256 2 /\
     lift_array256  res = ntt (dotp va vb)  ]  = 1%r by
